Move bitvector lemmas and tactics out of Expressions.v

vera/Bitvector.v
@@ -27,6 +27,9 @@ Local Open Scope bv_scope.
 
 Set Bullet Behavior "Strict Subproofs".
 
+#[global] Hint Rewrite Nat2N.id N2Nat.id @removelast_cons_length : xbv_size.
+Hint Rewrite Nat2N.inj_add Nat2N.inj_mul Nat2N.inj_sub Nat2N.inj_min Nat2N.inj_max : xbv_size.
+
 Module RawBV.
   Include RAWBITVECTOR_LIST.
   Notation t := bitvector.
@@ -62,6 +65,92 @@ Module RawBV.
     else bv_extr 0 width (size bv) bv.
 
   Definition to_N (val : bitvector) : N := N.of_nat (list2nat_be val).
+
+  Fixpoint to_string (val : bitvector) : string :=
+    match val with
+    | [] => ""
+    | b::bs => to_string bs ++ (if b then "1" else "0")
+    end.
+
+  Definition bv_map2_common_map2 (f : bool -> bool -> bool) (bv1 bv2 : bitvector) :
+    map2 f bv1 bv2 = (Common.map2 f bv1 bv2).
+  Proof.
+    generalize dependent bv2.
+    induction bv1; destruct bv2; intros; simp map2; try crush.
+  Qed.
+
+  Equations nice_nshl_be : list bool -> nat -> list bool :=
+    nice_nshl_be bs 0 := bs;
+    nice_nshl_be [] _ := [];
+    nice_nshl_be bs (S n) := false :: nice_nshl_be (List.removelast bs) n.
+
+  Lemma shl_be_nicify bs n :
+    nshl_be bs n = nice_nshl_be bs n.
+  Proof.
+    funelim (nice_nshl_be bs n); simp nice_nshl_be in *; simpl in *.
+    - reflexivity.
+    - induction n; crush.
+    - rewrite <- H. clear H Heqcall.
+      revert b l.
+      induction n; intros.
+      + crush.
+      + simpl.
+        now rewrite IHn.
+  Qed.
+
+  Equations nice_nshr_be : list bool -> nat -> list bool :=
+    nice_nshr_be [] _ := [];
+    nice_nshr_be bs 0 := bs;
+    nice_nshr_be (b :: bs) (S n) := nice_nshr_be bs n ++ [false].
+
+  Lemma shr_be_nicify bs n :
+    nshr_be bs n = nice_nshr_be bs n.
+  Proof.
+    funelim (nice_nshr_be bs n); simp nice_nshr_be in *; simpl in *.
+    - induction n; crush.
+    - reflexivity.
+    - rewrite <- H. clear b H Heqcall. revert bs.
+      induction n; intros; try crush.
+      simpl.
+      replace (_shr_be (bs ++ [false])) with (_shr_be bs ++ [false])%list
+        by (destruct bs; crush).
+      eapply IHn.
+  Qed.
+
+  (* bitvectors are little-endian, so shifts are inverted *)
+  Equations shl (bv : bitvector) (shamt : nat) : t :=
+    shl bv 0 := bv;
+    shl [] n := [];
+    shl bv (S n) := false :: shl (List.removelast bv) n
+  .
+
+  Lemma shl_size bv n : size (shl bv n) = size bv.
+  Proof.
+    unfold size. f_equal.
+    funelim (shl bv n);
+      try rewrite <- Heqcall in *; clear Heqcall;
+      [crush|crush|].
+    cbn [length]. f_equal. rewrite H.
+    apply removelast_cons_length.
+  Qed.
+
+  #[global] Hint Rewrite shl_size : xbv_size.
+
+  Equations shr (bv : bitvector) (shamt : nat) : bitvector :=
+    shr bv 0 := bv;
+    shr [] n := [];
+    shr (b :: bs) (S n) := shr bs n ++ [false]
+  .
+
+  Lemma shr_size bv n : size (shr bv n) = size bv.
+  Proof.
+    unfold size.
+    funelim (shr bv n); simp shr; try crush.
+    rewrite List.length_app.
+    crush.
+  Qed.
+
+  #[global] Hint Rewrite shr_size : xbv_size.
 
   Lemma pow2_pow i : pow2 i = 2 ^ i.
   Proof.
@@ -109,12 +198,12 @@ Module RawBV.
   Qed.
 
   Lemma _list2nat_be_zeros : forall w n i,
-      RawBV._list2nat_be (BVList.RAWBITVECTOR_LIST.mk_list_false w) n i = n.
+      _list2nat_be (BVList.RAWBITVECTOR_LIST.mk_list_false w) n i = n.
   Proof. induction w; crush. Qed.
 
   Lemma list2nat_be_zeros : forall w,
-      RawBV.list2nat_be (BVList.RAWBITVECTOR_LIST.mk_list_false w) = 0.
-  Proof. unfold RawBV.list2nat_be. intros. apply _list2nat_be_zeros. Qed.
+      list2nat_be (BVList.RAWBITVECTOR_LIST.mk_list_false w) = 0.
+  Proof. unfold list2nat_be. intros. apply _list2nat_be_zeros. Qed.
 
   Lemma list2nat_be_of_N_full v :
     list2nat_be (of_N_full v) = N.to_nat v.
@@ -170,102 +259,16 @@ Module RawBV.
     rewrite _list2nat_be_of_N_full.
     simpl. lia.
   Qed.
-
-  Fixpoint to_string (val : bitvector) : string :=
-    match val with
-    | [] => ""
-    | b::bs => to_string bs ++ (if b then "1" else "0")
-    end.
-
-  Definition bv_map2_common_map2 (f : bool -> bool -> bool) (bv1 bv2 : bitvector) :
-    map2 f bv1 bv2 = (Common.map2 f bv1 bv2).
-  Proof.
-    generalize dependent bv2.
-    induction bv1; destruct bv2; intros; simp map2; try crush.
-  Qed.
-
-  Equations nice_nshl_be : list bool -> nat -> list bool :=
-    nice_nshl_be bs 0 := bs;
-    nice_nshl_be [] _ := [];
-    nice_nshl_be bs (S n) := false :: nice_nshl_be (List.removelast bs) n.
-
-  Lemma shl_be_nicify bs n :
-    RawBV.nshl_be bs n = nice_nshl_be bs n.
-  Proof.
-    funelim (nice_nshl_be bs n); simp nice_nshl_be in *; simpl in *.
-    - reflexivity.
-    - induction n; crush.
-    - rewrite <- H. clear H Heqcall.
-      revert b l.
-      induction n; intros.
-      + crush.
-      + simpl.
-        now rewrite IHn.
-  Qed.
-
-  Equations nice_nshr_be : list bool -> nat -> list bool :=
-    nice_nshr_be [] _ := [];
-    nice_nshr_be bs 0 := bs;
-    nice_nshr_be (b :: bs) (S n) := nice_nshr_be bs n ++ [false].
-
-  Lemma shr_be_nicify bs n :
-    RawBV.nshr_be bs n = nice_nshr_be bs n.
-  Proof.
-    funelim (nice_nshr_be bs n); simp nice_nshr_be in *; simpl in *.
-    - induction n; crush.
-    - reflexivity.
-    - rewrite <- H. clear b H Heqcall. revert bs.
-      induction n; intros; try crush.
-      simpl.
-      replace (RawBV._shr_be (bs ++ [false])) with (RawBV._shr_be bs ++ [false])%list
-        by (destruct bs; crush).
-      eapply IHn.
-  Qed.
-
-  (* bitvectors are little-endian, so shifts are inverted *)
-  Equations shl (bv : bitvector) (shamt : nat) : t :=
-    shl bv 0 := bv;
-    shl [] n := [];
-    shl bv (S n) := false :: shl (List.removelast bv) n
-  .
-
-  Lemma shl_size bv n : size (shl bv n) = size bv.
-  Proof.
-    unfold size. f_equal.
-    funelim (shl bv n);
-      try rewrite <- Heqcall in *; clear Heqcall;
-      [crush|crush|].
-    cbn [length]. f_equal. rewrite H.
-    apply removelast_cons_length.
-  Qed.
-
-  Equations shr (bv : bitvector) (shamt : nat) : bitvector :=
-    shr bv 0 := bv;
-    shr [] n := [];
-    shr (b :: bs) (S n) := shr bs n ++ [false]
-  .
-
-  Lemma shr_size bv n : size (shr bv n) = size bv.
-  Proof.
-    unfold size.
-    funelim (shr bv n); simp shr; try crush.
-    rewrite List.length_app.
-    crush.
-  Qed.
 End RawBV.
 
 Module BV.
   Include BITVECTOR_LIST.
 
-  Program Definition ones (n : N) : bitvector n :=
-    {|
-      bv := RawBV.ones n;
-    |}.
-  Next Obligation.
-    unfold RawBV.ones, RawBV.size.
-    rewrite List.repeat_length.
-    apply N2Nat.id.
-  Qed.
+  Definition is_zero {n} (bv : bitvector n) : bool :=
+    bv_eq bv (zeros n).
+
+  Definition to_N {n} (bv : bitvector n) : N :=
+    RawBV.to_N (bits bv).
 
   Lemma of_bits_equal n (bv1 bv2 : bitvector n) :
     bits bv1 = bits bv2 ->
@@ -281,11 +284,34 @@ Module BV.
     apply RAWBITVECTOR_LIST.List_eq_refl.
   Qed.
 
-  Definition is_zero {n} (bv : bitvector n) : bool :=
-    bv_eq bv (zeros n).
+  (* Local variant of the tactic. The full version needs XBV so it
+    can't be defined here *)
+  #[local]
+  Ltac bitvector_erase :=
+    repeat match goal with
+           | [ bv : bitvector _ |- _ ] => destruct bv
+           | [ H : ?xbv1 = ?xbv2 |- _ ] =>
+  	   match type of xbv1 with
+  	   | bitvector _ =>
+  	     apply (f_equal bits) in H; simpl in H
+             end
+           | [ |- ?xbv1 = ?xbv2] =>
+  	   match type of xbv1 with
+  	   | bitvector _ => apply of_bits_equal; simpl
+             end
+           | [ |- context[rew _ in _] ] => destruct_rew
+  	 end;
+    unfold to_N in *; simpl in *.
 
-  Definition to_N {n} (bv : bitvector n) : N :=
-    RawBV.to_N (bits bv).
+  Program Definition ones (n : N) : bitvector n :=
+    {|
+      bv := RawBV.ones n;
+    |}.
+  Next Obligation.
+    unfold RawBV.ones, RawBV.size.
+    rewrite List.repeat_length.
+    apply N2Nat.id.
+  Qed.
 
   Lemma to_N_max_bound n (b : bitvector n) : (to_N b < 2 ^ n)%N.
   Proof.
@@ -302,11 +328,11 @@ Module BV.
   Qed.
 
   Lemma bv_zextn_to_N n w (bv : bitvector n):
-    BV.to_N (BV.bv_concat (BV.zeros w) bv) =
-      BV.to_N bv.
+    to_N (bv_concat (zeros w) bv) =
+      to_N bv.
   Proof.
     destruct bv.
-    unfold BV.to_N, RawBV.to_N, BV.bv_concat, RawBV.bv_concat, BV.zeros, RawBV.zeros.
+    unfold to_N, RawBV.to_N, bv_concat, RawBV.bv_concat, zeros, RawBV.zeros.
     f_equal. simpl.
     rewrite RawBV.list2nat_be_cons.
     rewrite RawBV.list2nat_be_zeros.
@@ -339,14 +365,97 @@ Module BV.
 
   #[program]
   Definition shl {n} (bv : bitvector n) (shamt : N) : bitvector n :=
-    {| bv := RawBV.shl (BV.bits bv) (N.to_nat shamt) |}.
+    {| bv := RawBV.shl (bits bv) (N.to_nat shamt) |}.
   Next Obligation. rewrite RawBV.shl_size. apply wf. Qed.
 
   #[program]
   Definition shr {n} (bv : bitvector n) (shamt : N) : bitvector n :=
-    {| bv := RawBV.shr (BV.bits bv) (N.to_nat shamt) |}.
+    {| bv := RawBV.shr (bits bv) (N.to_nat shamt) |}.
   Next Obligation. rewrite RawBV.shr_size. apply wf. Qed.
 
+  Lemma shr_swap_definition w lhs rhs :
+    bv_shr (n:=w) lhs rhs = shr lhs (to_N rhs).
+  Proof.
+   bitvector_erase.
+   unfold RawBV.bv_shr, RawBV.to_N in *.
+   rewrite wf0, wf1, N.eqb_refl, Nat2N.id in *.
+   clear wf0 wf1.
+   unfold RawBV.shr_be.
+   rewrite RawBV.shr_be_nicify.
+   generalize dependent (RawBV.list2nat_be bv0).
+   intros shamt. clear w bv0.
+   unfold RawBV.size in *.
+   funelim (RawBV.shr bv1 shamt).
+   - destruct bv0; simp nice_nshr_be; reflexivity.
+   - simp nice_nshr_be. crush.
+   - simp nice_nshr_be. crush.
+  Qed.
+  
+  Lemma shl_swap_definition w lhs rhs :
+    bv_shl (n:=w) lhs rhs = shl lhs (to_N rhs).
+  Proof.
+   bitvector_erase.
+   unfold RawBV.bv_shl, RawBV.to_N in *.
+   rewrite wf0, wf1, N.eqb_refl, Nat2N.id in *.
+   clear wf0 wf1.
+   unfold RawBV.shl_be.
+   rewrite RawBV.shl_be_nicify.
+   generalize dependent (RawBV.list2nat_be bv0).
+   intros shamt. clear w bv0.
+   unfold RawBV.size in *.
+   funelim (RawBV.shl bv1 shamt).
+   - destruct bv0; simp nice_nshl_be; reflexivity.
+   - simp nice_nshl_be. crush.
+   - simp nice_nshl_be. crush.
+  Qed.
+  
+  Lemma bv_extr_one_bit (n : N) w (bv : bitvector w) :
+    (1 + n <= w)%N ->
+    bv_extr n 1 bv = of_bits [bitOf (N.to_nat n) bv].
+  Proof.
+    destruct bv as [bv wf].
+    subst. intros.
+    apply of_bits_equal.
+    simpl.
+    unfold bv_extr, RawBV.bv_extr, RawBV.size in *.
+    autodestruct_eqn E; try (rewrite N.ltb_lt in *; lia); clear E.
+    replace (N.to_nat (1 + n)) with (S (N.to_nat n)) by lia.
+    assert (S (N.to_nat n) <= List.length bv) as H' by lia. clear H. revert H'.
+    generalize (N.to_nat n). clear n. intros n H.
+    revert bv H.
+    induction n; intros.
+    { destruct bv0; try crush.
+      destruct bv0; crush.
+    }
+    destruct bv0; try crush.
+    simpl.
+    rewrite IHn; crush.
+  Qed.
+
+  Lemma bv_shr_as_select w (vec : bitvector w) (idx : bitvector w) :
+    (w > 0)%N ->
+    bv_extr 0 1 (bv_shr vec idx) =
+      of_bits [bitOf (N.to_nat (to_N idx)) vec]%list.
+  Proof.
+    intros Hbound.
+    rewrite bv_extr_one_bit; try crush.
+    apply of_bits_equal. simpl.
+    do 2 f_equal.
+    unfold bitOf, bv_shr.
+    destruct vec as [vec vec_wf].
+    destruct idx as [idx idx_wf].
+    simpl.
+    unfold to_N, RawBV.to_N, bv_shr, RawBV.bv_shr, RawBV.shr_be, RawBV.size in *.
+    simpl.
+    rewrite vec_wf, idx_wf, N.eqb_refl.
+    generalize (RawBV.list2nat_be idx). clear idx idx_wf. intro n.
+    destruct n, vec; try crush.
+    unfold RawBV.bitOf.
+    rewrite RawBV.shr_be_nicify. simp nice_nshr_be. rewrite Nat2N.id. simpl.
+    clear b vec_wf.
+    funelim (RawBV.nice_nshr_be vec n); simp nice_nshr_be; try crush.
+    destruct (RawBV.nice_nshr_be bs n); crush.
+  Qed.
 End BV.
 
 Module RawXBV.
@@ -380,6 +489,14 @@ Module RawXBV.
 
   Arguments size / _.
 
+  Lemma fold_size bv : N.of_nat (List.length bv) = size bv.
+  Proof. reflexivity. Qed.
+  
+  Lemma removelast_cons_size b bs : size (List.removelast (b :: bs)) = size bs.
+  Proof. unfold size. now rewrite removelast_cons_length. Qed.
+  
+  #[global] Hint Rewrite fold_size removelast_cons_size : xbv_size.
+
   Definition exes (count : N) : xbv := List.repeat X (nat_of_N count).
   Definition zeros (count : N) : xbv := List.repeat O (nat_of_N count).
   Definition ones (count : N) : xbv := List.repeat I (nat_of_N count).
@@ -393,6 +510,8 @@ Module RawXBV.
       lia.
   Qed.
 
+  #[global] Hint Rewrite @exes_size : xbv_size.
+
   Lemma ones_size {n} : size (ones n) = n.
   Proof.
     unfold ones.
@@ -402,6 +521,8 @@ Module RawXBV.
       lia.
   Qed.
 
+  #[global] Hint Rewrite @ones_size : xbv_size.
+
   Lemma zeros_size {n} : size (zeros n) = n.
   Proof.
     unfold zeros.
@@ -410,6 +531,8 @@ Module RawXBV.
     - rewrite Nnat.N2Nat.inj_succ. simpl in *.
       lia.
   Qed.
+
+  #[global] Hint Rewrite @zeros_size : xbv_size.
 
   Definition bit_eq_dec (b1 b2: bit) : { b1 = b2 } + { b1 <> b2 }.
   Proof. unfold decidable. decide equality. Qed.
@@ -428,6 +551,8 @@ Module RawXBV.
     induction bv; simpl; lia.
   Qed.
 
+  #[global] Hint Rewrite @from_bv_size : xbv_size.
+
   Definition to_bv (bv : xbv) : option RawBV.t :=
     mapT bit_to_bool bv
   .
@@ -444,6 +569,8 @@ Module RawXBV.
       cbn. lia.
   Qed.
 
+  #[global] Hint Rewrite @to_bv_size : xbv_size.
+
   Definition replicate (n : N) (b : bit) :=
     List.repeat b (N.to_nat n).
 
@@ -454,6 +581,8 @@ Module RawXBV.
     rewrite List.repeat_length.
     apply N2Nat.id.
   Qed.
+
+  #[global] Hint Rewrite @replicate_size : xbv_size.
 
   Definition has_x (bv : xbv) : Prop :=
     List.Exists (fun b => b = X) bv.
@@ -535,33 +664,46 @@ Module RawXBV.
     end
   .
 
-  (* Definition from_sized_bv {w} (bv : BV.bitvector w) : xbv := *)
-  (*   from_bv (BV.bits bv). *)
-
-  (* Definition to_sized_bv (v : xbv) : option (BV.bitvector (size v)) := *)
-  (*   match to_bv v as x return _ = x -> _ with *)
-  (*   | Some bv => fun e => Some {| BV.bv := bv; BV.wf := to_bv_size xbv bv e |} *)
-  (*   | None => fun e => None *)
-  (*   end eq_refl. *)
-
-  (* Import EqNotations. *)
-
   Equations to_bv_same_width (l r : xbv) : option (RawBV.t * RawBV.t) :=
     to_bv_same_width l r with dec (size r = size l), to_bv l, to_bv r => {
       | left e, Some l_bv, Some r_bv => Some (l_bv, r_bv)
       | _, _, _ => None
       }.
 
-  (* Equations to_sized_bv_same_width (l r : t) : option (BV.bitvector (size l) * BV.bitvector (size l)) := *)
-  (*   to_sized_bv_same_width l r with dec (size r = size l), to_sized_bv l, to_sized_bv r => { *)
-  (*     | left e, Some l_bv, Some r_bv => Some (l_bv, rew e in r_bv) *)
-  (*     | _, _, _ => None *)
-  (*     }. *)
-
   Definition concat (l r : xbv) : xbv := r ++ l.
 
   Lemma concat_size {l r} : size (concat l r) = (size l + size r)%N.
   Proof. unfold concat, size. rewrite List.length_app. lia. Qed.
+
+  #[global] Hint Rewrite @concat_size : xbv_size.
+
+  Lemma concat_empty1 (x1 x2 : xbv) :
+    (size x1 = 0)%N ->
+    concat x1 x2 = x2.
+  Proof.
+    intros. unfold concat, size in *.
+    destruct x1; [|simpl in H; lia].
+    now rewrite List.app_nil_r.
+  Qed.
+
+  Lemma concat_empty2 (x1 x2 : xbv) :
+    (size x2 = 0)%N ->
+    concat x1 x2 = x1.
+  Proof.
+    intros. unfold concat, size in *.
+    destruct x2; [reflexivity|simpl in H; lia].
+  Qed.
+
+  Lemma concat_assoc (x1 x2 x3 : xbv) :
+    concat x1 (concat x2 x3) = concat (concat x1 x2) x3.
+  Proof. unfold concat. now rewrite List.app_assoc. Qed.
+
+  Lemma concat_zeros (w1 w2 : N) :
+    concat (zeros w1) (zeros w2) = zeros (w1 + w2).
+  Proof.
+    unfold zeros, concat.
+    rewrite <- List.repeat_app. f_equal. lia.
+  Qed.
 
   Equations extract (x: xbv) (i j: nat) : xbv :=
     extract [] i j := [];
@@ -576,11 +718,15 @@ Module RawXBV.
       simp extract; simpl in *; try crush.
   Qed.
 
+  #[global] Hint Rewrite @extract_width : xbv_size.
+
   Lemma extract_size x i j :
     size (extract x (N.to_nat i) (N.to_nat j)) = (N.min j (size x - i))%N.
   Proof.
     unfold size. rewrite extract_width. lia.
   Qed.
+
+  #[global] Hint Rewrite @extract_size : xbv_size.
 
   Definition extr (v : xbv) (i j : N) : xbv :=
     if (j + i <=? size v)%N
@@ -596,6 +742,8 @@ Module RawXBV.
       rewrite extract_width; try crush.
     - apply exes_size.
   Qed.
+
+  #[global] Hint Rewrite @extr_width : xbv_size.
 
   Definition bitOf (n : nat) (v: xbv): bit := nth n v X.
 
@@ -613,6 +761,8 @@ Module RawXBV.
         replace (List.mapT_list bit_to_bool (from_bv bv)) with (Some bv).
         reflexivity.
   Qed.
+
+  #[global] Hint Rewrite @xbv_bv_inverse : xbv_size.
 
   Lemma bv_xbv_inverse : forall x bv,
       to_bv x = Some bv ->
@@ -645,6 +795,24 @@ Module RawXBV.
     apply removelast_cons_length.
   Qed.
 
+  #[global] Hint Rewrite @shl_size : xbv_size.
+
+  Lemma shl_overshift xbv shamt :
+    (N.of_nat shamt >= size xbv)%N ->
+    shl xbv shamt = zeros (size xbv).
+  Proof.
+    intros.
+    unfold size, zeros in *.
+    N_to_nat.
+    funelim (shl xbv shamt).
+    - destruct bv; crush.
+    - reflexivity.
+    - cbn [List.length] in *.
+      erewrite H by (rewrite removelast_cons_length; crush).
+      rewrite removelast_cons_length.
+      crush.
+  Qed.
+
   Equations shr (bv : xbv) (shamt : nat) : xbv :=
     shr bv 0 := bv;
     shr [] n := [];
@@ -658,6 +826,23 @@ Module RawXBV.
     funelim (shr bv n); simp shr; try crush.
     rewrite List.length_app.
     crush.
+  Qed.
+
+  #[global] Hint Rewrite @shr_size : xbv_size.
+
+  Lemma shr_overshift xbv shamt :
+    (N.of_nat shamt >= size xbv)%N ->
+    shr xbv shamt = zeros (size xbv).
+  Proof.
+    intros.
+    unfold size, zeros in *.
+    N_to_nat.
+    funelim (shr xbv shamt).
+    - destruct bv; crush.
+    - reflexivity.
+    - cbn [List.length] in *.
+      rewrite H by lia. clear H H0 Heqcall.
+      induction (List.length bs); crush.
   Qed.
 
   (*
@@ -680,6 +865,321 @@ Module RawXBV.
     mk_dec_eq.
 
   Global Instance dec_has_x xbv : DecProp (has_x xbv) := _.
+
+  Lemma extract_full w (xbv : xbv) :
+    w = N.to_nat (size xbv) ->
+    extract xbv 0 w = xbv.
+  Proof.
+    intros.
+    subst. unfold size. rewrite Nat2N.id.
+    funelim (extract xbv 0 (List.length xbv)); crush.
+  Qed.
+  
+  Lemma extract_empty lo sz (xbv : xbv) :
+    sz = 0 ->
+    extract xbv lo sz = [].
+  Proof.
+    intros. subst.
+    funelim (extract xbv lo 0); crush.
+  Qed.
+  
+  Lemma extr_empty lo sz (xbv : xbv) :
+    (sz = 0)%N ->
+    extr xbv lo sz = [].
+  Proof.
+    intros. subst. unfold extr.
+    rewrite extract_empty by lia.
+    unfold exes; simpl. crush.
+  Qed.
+
+  Lemma shr_as_concat_gt (n : nat) (xbv : xbv) :
+    (List.length xbv < n) ->
+    shr xbv n = zeros (size xbv).
+  Proof.
+    funelim (shr xbv n); intros; unfold zeros; simpl in *.
+    - destruct bv; crush.
+    - reflexivity.
+    - insterU H.
+      unfold zeros in *.
+      rewrite Pnat.SuccNat2Pos.id_succ.
+      rewrite Nat2N.id in *.
+      simpl. rewrite H.
+      clear Heqcall H0 H.
+      induction (List.length bs); crush.
+  Qed.
+  
+  Lemma shr_as_concat_le (n : nat) (xbv : xbv) :
+    (n <= List.length xbv) ->
+    shr xbv n =
+      concat
+        (zeros (N.of_nat n))
+        (extr xbv (N.of_nat n) (size xbv - N.of_nat n)).
+  Proof.
+    unfold zeros, concat, extr, size.
+    simpl. rewrite Nat2N.id.
+    intros.
+    autodestruct_eqn E; kill_bools; try lia.
+    funelim (shr xbv n); [idtac|crush|idtac].
+    + simpl in *.
+      rewrite extract_full. 
+      * now rewrite List.app_nil_r. 
+      * unfold size. lia.
+    + insterU H. simp extract.
+      rewrite H. clear H.
+      rewrite ! N2Nat.inj_sub, ! Nat2N.id.
+      simpl.
+      rewrite <- List.app_assoc. f_equal.
+      clear E H0 Heqcall. induction n; crush.
+  Qed.
+  
+  Lemma shr_as_concat (n : nat) (xbv : xbv) :
+    shr xbv n =
+      concat
+        (zeros (N.of_nat (min (List.length xbv) n)))
+        (extr xbv (N.of_nat n) (size xbv - N.of_nat n)).
+  Proof.
+    destruct (Nat.leb n (List.length xbv)) eqn:E; kill_bools.
+    - rewrite Nat.min_r by lia.
+      apply shr_as_concat_le. lia.
+    - rewrite Nat.min_l by lia.
+      rewrite shr_as_concat_gt by lia.
+      unfold extr.
+      autodestruct_eqn Hcmp; kill_bools; [crush|clear Hcmp].
+      rewrite concat_empty2. reflexivity.
+      rewrite exes_size. unfold size. lia.
+  Qed.
+  
+  Lemma shl_as_concat_gt (n : nat) (xbv : xbv) :
+    (List.length xbv < n) ->
+    shl xbv n = zeros (size xbv).
+  Proof.
+    funelim (shl xbv n); intros.
+    - destruct bv; crush.
+    - reflexivity.
+    - insterU H.
+      autorewrite with xbv_size in *.
+      unfold size, zeros in *.
+      cbn [List.length] in *. 
+      erewrite H by lia.
+      rewrite ! Nat2N.id. reflexivity.
+  Qed.
+  
+  Lemma extract_remove_last n l:
+    n < List.length l ->
+    extract (List.removelast l) 0 n = extract l 0 n.
+  Proof.
+    revert n.
+    induction l; intros.
+    - destruct n; [|crush]. reflexivity.
+    - simpl in H.
+      destruct n; [rewrite ! extract_empty; crush|].
+      simp extract. destruct l; [crush|].
+      simpl. simp extract.
+      f_equal. apply IHl. lia.
+  Qed.
+  
+  Lemma shl_as_concat_le (n : nat) (xbv : xbv) :
+    (n <= List.length xbv) ->
+    shl xbv n =
+      concat
+        (extr xbv 0 (size xbv - N.of_nat n))
+        (zeros (N.of_nat n)).
+  Proof.
+    unfold zeros, concat, extr, size.
+    simpl. rewrite Nat2N.id.
+    intros.
+    autodestruct_eqn E; kill_bools; N_to_nat; try lia.
+    funelim (shl xbv n); [idtac|crush|idtac].
+    + simpl in *.
+      rewrite extract_full. 
+      * reflexivity.
+      * unfold size. lia.
+    + insterU H. simp extract.
+      rewrite H by (autorewrite with xbv_size in *; crush).
+      clear H. cbn [List.repeat List.app]. do 2 f_equal.
+      autorewrite with xbv_size.
+      apply extract_remove_last.
+      lia.
+  Qed.
+  
+  Lemma shl_as_concat (n : nat) (xbv : xbv) :
+    shl xbv n =
+      concat
+        (extr xbv 0 (size xbv - N.of_nat n))
+        (zeros (N.of_nat (min (List.length xbv) n)))
+        .
+  Proof.
+    destruct (Nat.leb n (List.length xbv)) eqn:E; kill_bools.
+    - rewrite Nat.min_r by lia.
+      apply shl_as_concat_le. lia.
+    - rewrite Nat.min_l by lia.
+      rewrite shl_as_concat_gt by lia.
+      unfold extr.
+      autodestruct_eqn Hcmp; kill_bools; [|crush].
+      rewrite concat_empty1. reflexivity.
+      autorewrite with xbv_size. unfold size in *. lia.
+  Qed.
+  
+  Lemma extr_of_concat_lo xbv_hi xbv_lo lo sz :
+    (lo <= size xbv_lo)%N ->
+    (lo + sz <= size xbv_lo)%N ->
+    extr (concat xbv_hi xbv_lo) lo sz = extr xbv_lo lo sz.
+  Proof.
+    intros Hlo Hhi.
+    unfold extr.
+    autodestruct_eqn E; kill_bools;
+      autorewrite with xbv_size in *;
+      try lia; [idtac].
+    clear E E0.
+    N_to_nat. unfold concat.
+    funelim (extract xbv_lo lo sz).
+    - simpl in *.
+      replace i with 0 by lia.
+      replace j with 0 by lia. 
+      destruct xbv_hi; simp extract; reflexivity.
+    - simpl in *. simp extract. reflexivity.
+    - simpl in *. simp extract.
+      erewrite H; try crush.
+    - simpl in *. simp extract. eapply H; lia.
+  Qed.
+  
+  Lemma extr_of_concat_hi xbv_hi xbv_lo lo sz :
+    (size xbv_lo <= lo)%N ->
+    (lo + sz <= size xbv_lo + size xbv_hi)%N ->
+    extr (concat xbv_hi xbv_lo) lo sz =
+      extr xbv_hi (lo - size xbv_lo) sz.
+  Proof.
+    intros Hlo Hhi.
+    unfold extr.
+    autodestruct_eqn E; kill_bools;
+      autorewrite with xbv_size in *;
+      try lia; [idtac].
+    clear E E0.
+    unfold size, concat in *.
+    N_to_nat.
+    funelim (extract (xbv_lo ++ xbv_hi) lo sz); intros.
+    - symmetry in H. apply List.app_eq_nil in H.
+      destruct H. subst. simp extract. reflexivity.
+    - destruct xbv_lo; [|crush]. simpl.
+      destruct xbv_hi; now simp extract.
+    - destruct xbv_lo; [|crush]. simpl in *. subst.
+      simp extract. reflexivity.
+    - destruct xbv_lo; simpl in *.
+      + subst. simp extract. reflexivity.
+      + inv H0. eapply H; crush.
+  Qed.
+  
+  Lemma extr_of_concat_mid xbv_hi xbv_lo lo sz :
+    (lo <= size xbv_lo)%N ->
+    (size xbv_lo <= lo + sz)%N ->
+    (lo + sz <= size xbv_lo + size xbv_hi)%N ->
+    extr (concat xbv_hi xbv_lo) lo sz =
+      concat
+        (extr xbv_hi (lo - size xbv_lo)%N (sz - (size xbv_lo - lo))%N)
+        (extr xbv_lo lo (size xbv_lo - lo)%N).
+  Proof.
+    intros Hlo Hmid Hhi.
+    unfold extr.
+    autodestruct_eqn E; kill_bools;
+      autorewrite with xbv_size in *;
+      try lia; [idtac].
+    clear E E0 E1.
+    unfold size, concat in *.
+    N_to_nat.
+    funelim (extract (xbv_lo ++ xbv_hi) lo sz); intros.
+    - symmetry in H. apply List.app_eq_nil in H.
+      destruct H. subst. simp extract. reflexivity.
+    - destruct xbv_lo; [|crush]. simpl.
+      destruct xbv_hi; now simp extract.
+    - destruct xbv_lo.
+      + simpl in *. subst. simpl. simp extract. simpl.
+        repeat f_equal.
+      + simpl in *. inv H0. simp extract. simpl. f_equal.
+        erewrite H by crush.
+        repeat f_equal; try crush.
+    - destruct xbv_lo; [crush|]. simpl in *. simp extract.
+      inv H0. erewrite H by crush.
+      f_equal.
+  Qed.
+  
+  Lemma extr_of_concat xbv_hi xbv_lo lo sz :
+    (lo + sz <= size xbv_hi + size xbv_lo)%N ->
+    extr (concat xbv_hi xbv_lo) lo sz =
+      concat
+        (extr xbv_hi (lo - size xbv_lo) (sz - (size xbv_lo - lo)))%N
+        (extr xbv_lo lo (N.min sz (size xbv_lo - lo)))%N.
+  Proof.
+    intros.
+    destruct (dec (size xbv_lo <= lo)%N);
+      destruct (dec (lo + sz < size xbv_lo))%N; try lia.
+    - replace (N.min sz (size xbv_lo - lo)) with (size xbv_lo - lo)%N by lia.
+      replace (size xbv_lo - lo)%N with 0%N by lia.
+      erewrite extr_of_concat_hi by lia.
+      rewrite concat_empty2 by (autorewrite with xbv_size; lia).
+      f_equal. lia.
+    - replace (N.min sz (size xbv_lo - lo)) with sz by lia.
+      replace (sz - (size xbv_lo - lo))%N with 0%N by lia.
+      erewrite extr_of_concat_lo by lia.
+      rewrite concat_empty1 by (autorewrite with xbv_size; lia).
+      reflexivity.
+    - replace (N.min sz (size xbv_lo - lo)) with (size xbv_lo - lo)%N by lia.
+      eapply extr_of_concat_mid; lia.
+  Qed.
+  
+  Lemma extr_of_zeros w lo sz :
+    (lo + sz <= w)%N ->
+    extr (zeros w) lo sz = zeros sz.
+  Proof.
+    intros. unfold extr.
+    autorewrite with xbv_size.
+    autodestruct_eqn E; kill_bools; [clear E|crush].
+    unfold zeros.
+    N_to_nat.
+    revert lo sz H.
+    induction w; intros; simpl; simp extract.
+    - replace sz with 0; crush.
+    - destruct lo, sz; simpl; simp extract.
+      + reflexivity.
+      + erewrite IHw; crush.
+      + erewrite IHw; crush.
+      + erewrite IHw; crush.
+  Qed.
+  
+  Lemma extr_of_extr lo1 lo2 sz1 sz2 xbv :
+    (lo1 + sz1 <= size xbv)%N ->
+    (lo2 + sz2 <= sz1)%N ->
+    extr (extr xbv lo1 sz1) lo2 sz2 = extr xbv (lo1 + lo2) sz2.
+  Proof.
+    intros H0 H1.
+    unfold extr.
+    autodestruct_eqn E;
+      autorewrite with xbv_size kill_bools in *;
+      try crush; N_to_nat.
+    clear E E0 E1.
+    revert sz1 H0 H1.
+    funelim (extract xbv (lo1 + lo2) sz2).
+    - intros. simp extract. reflexivity.
+    - intros.
+      replace lo2 with 0 in * by lia.
+      destruct (extract (bx :: x') lo1 sz1); simp extract; reflexivity.
+    - intros. simpl in *. clear Heqcall.
+      replace lo1 with 0 in * by crush.
+      replace lo2 with 0 in * by crush.
+      destruct sz1; [lia|].
+      simp extract.
+      erewrite H; crush.
+    - intros. simpl in *. clear Heqcall.
+      destruct lo1, sz1;
+        simpl in *; subst; simp extract.
+      + lia.
+      + erewrite H; crush.
+      + erewrite H; crush.
+      + erewrite H; crush.
+  Qed.
+
+  Lemma from_bv_app b1 b2 :
+    from_bv (b1 ++ b2)%list = (from_bv b1 ++ from_bv b2)%list.
+  Proof. unfold from_bv. apply List.map_app. Qed.
 End RawXBV.
 
 Module XBV.
@@ -861,6 +1361,30 @@ Module XBV.
     apply BV.to_N_max_bound.
   Qed.
 
+  #[global]
+  Ltac bitvector_erase :=
+    repeat match goal with
+           | [ xbv : xbv _ |- _ ] => destruct xbv
+           | [ bv : BV.bitvector _ |- _ ] => destruct bv
+           | [ H : RawXBV.size ?xbv = 0%N |- _ ] =>
+  	   destruct xbv; [|discriminate]; clear H; simpl in *
+           | [ H : to_bv _ = None |- _ ] => rewrite <- has_x_to_bv in H
+           | [ H : ?xbv1 = ?xbv2 |- _ ] =>
+  	   match type of xbv1 with
+  	   | xbv _ =>
+  	     apply (f_equal bits) in H; simpl in H
+  	   | BV.bitvector _ =>
+  	     apply (f_equal BV.bits) in H; simpl in H
+             end
+           | [ |- ?xbv1 = ?xbv2] =>
+  	   match type of xbv1 with
+  	   | xbv _ => apply of_bits_equal; simpl
+  	   | BV.bitvector _ => apply BV.of_bits_equal; simpl
+             end
+           | [ |- context[rew _ in _] ] => destruct_rew
+  	 end;
+    unfold has_x, BV.to_N in *; simpl in *.
+
   Definition extr {n} (x: xbv n) (i j: N) : xbv j :=
     {|
       bv := RawXBV.extr (bits x) i j;
@@ -915,6 +1439,22 @@ Module XBV.
     apply of_bits_equal; simpl.
     unfold RAWBITVECTOR_LIST.bv_concat, RawXBV.from_bv.
     now rewrite map_app.
+  Qed.
+
+  Lemma concat_no_exes n1 n2 (bv1 : BV.bitvector n1) (bv2 : BV.bitvector n2) :
+    concat (from_bv bv1) (from_bv bv2) = from_bv (BV.bv_concat bv1 bv2).
+  Proof.
+    destruct bv1 as [bv1 wf1], bv2 as [bv2 wf2].
+    apply of_bits_equal. simpl.
+    unfold RawBV.bv_concat, RawXBV.from_bv.
+    rewrite List.map_app.
+    reflexivity.
+  Qed.
+
+  Lemma concat_empty1 {w} (x1 : xbv 0) (x2 : xbv w) :
+    rew [xbv] (N.add_0_l w) in concat x1 x2 = x2.
+  Proof.
+    bitvector_erase. unfold RawXBV.concat. now rewrite List.app_nil_r.
   Qed.
 
   Program Definition replicate (n : N) (b : bit) : xbv n :=
@@ -978,13 +1518,31 @@ Module XBV.
 
   #[program]
   Definition shl {n} (bv : xbv n) (shamt : N) : xbv n :=
-    {| bv := RawXBV.shl (XBV.bits bv) (N.to_nat shamt) |}.
+    {| bv := RawXBV.shl (bits bv) (N.to_nat shamt) |}.
   Next Obligation. rewrite RawXBV.shl_size. apply wf. Qed.
+
+  Lemma shl_overshift {n} (x : xbv n) shamt :
+    (shamt >= n)%N ->
+    shl x shamt = zeros n.
+  Proof.
+    intros.
+    bitvector_erase. subst.
+    erewrite RawXBV.shl_overshift; unfold RawXBV.size in *; crush.
+  Qed.
 
   #[program]
   Definition shr {n} (bv : xbv n) (shamt : N) : xbv n :=
-    {| bv := RawXBV.shr (XBV.bits bv) (N.to_nat shamt) |}.
+    {| bv := RawXBV.shr (bits bv) (N.to_nat shamt) |}.
   Next Obligation. rewrite RawXBV.shr_size. apply wf. Qed.
+
+  Lemma shr_overshift {n} (x : xbv n) shamt :
+    (shamt >= n)%N ->
+    shr x shamt = zeros n.
+  Proof.
+    intros.
+    bitvector_erase. subst.
+    erewrite RawXBV.shr_overshift; unfold RawXBV.size in *; crush.
+  Qed.
 
   (*
    * Matches this Verilog operation:
@@ -1010,4 +1568,314 @@ Module XBV.
 
   #[global]
   Instance dec_has_x {n} (x : xbv n) : DecProp (has_x x) := _.
+
+  Lemma shl_to_bv n vec shamt :
+    to_bv (shl (from_bv vec) shamt) = Some (BV.shl (n:=n) vec shamt).
+  Proof.
+    unfold BV.to_N, BV.shl.
+    intros.
+    destruct vec as [vec vec_wf].
+    rewrite <- xbv_bv_inverse. f_equal.
+    apply of_bits_equal; simpl.
+    generalize dependent (N.to_nat shamt). clear shamt. intro shamt.
+    funelim (RawBV.shl vec shamt).
+    - reflexivity.
+    - reflexivity.
+    - insterU H.
+      unfold RawXBV.from_bv in *. cbn [List.map].
+      simp shl. repeat f_equal.
+      rewrite map_removelast in *.
+      cbn [List.map] in H.
+      apply H.
+  Qed.
+  
+  Lemma shr_to_bv n vec shamt :
+    to_bv (shr (from_bv vec) shamt) = Some (BV.shr (n:=n) vec shamt).
+  Proof.
+    unfold BV.to_N, BV.shr.
+    intros.
+    destruct vec as [vec vec_wf].
+    rewrite <- xbv_bv_inverse. f_equal.
+    apply of_bits_equal; simpl.
+    generalize dependent (N.to_nat shamt). clear shamt. intro shamt.
+    funelim (RawBV.shr vec shamt); simpl; simp shr.
+    - reflexivity.
+    - reflexivity.
+    - unfold RawXBV.from_bv in *.
+      rewrite List.map_app. simpl. repeat f_equal.
+      eauto.
+  Qed.
+
+  Lemma bitOf_in_bounds n w (bv : BV.bitvector w) def :
+    (n < w)%N ->
+    RawXBV.bit_to_bool (bitOf (N.to_nat n) (from_bv bv)) = Some (List.nth (N.to_nat n) (BV.bits bv) def).
+  Proof.
+    intros H.
+    destruct bv as [bv wf].
+    unfold from_bv, RawXBV.from_bv, bitOf, RawXBV.bitOf,
+      BVList.RAWBITVECTOR_LIST.size in *.
+    subst. simpl.
+    erewrite List.nth_indep
+      by (rewrite List.length_map; lia).
+    rewrite List.map_nth.
+    rewrite RawXBV.bit_to_bool_inverse.
+    reflexivity.
+  Qed.
+
+  Lemma to_bv_some_raw_iff w (xbv : xbv w) (bv : BV.bitvector w) :
+    to_bv xbv = Some bv <-> RawXBV.to_bv (bits xbv) = Some (BV.bits bv).
+  Proof.
+    (* This is disgusting (written while half asleep) plzfix *)
+    split; intros; simpl in *.
+    - apply bv_xbv_inverse in H. subst.
+      destruct bv as [bv bv_wf].
+      simpl. apply RawXBV.xbv_bv_inverse.
+    - apply RawXBV.bv_xbv_inverse in H.
+      destruct bv as [bv bv_wf].
+      simpl in *.
+      funelim (to_bv xbv).
+      + unfold raw_to_bv_with_proof in *.
+        rewrite e in Heq. inv Heq.
+        f_equal.
+        apply BV.of_bits_equal.
+        simpl. destruct_rew.
+        destruct v as [v v_wf].
+        unfold bits, bv, RawBV.of_bits in *. simpl in *. subst.
+        rewrite RawXBV.xbv_bv_inverse in e.
+        inv e.
+        reflexivity.
+      + destruct v as [v v_wf].
+        simpl in *. subst.
+        clear Heq.
+        rewrite RawXBV.xbv_bv_inverse in prf.
+        discriminate.
+  Qed.
+
+  Lemma concat_from_bv_inv1 n1 n2 (xbv1 : xbv n1) (xbv2 : xbv n2) bv :
+    concat xbv1 xbv2 = from_bv bv ->
+    (exists bv1, xbv1 = from_bv bv1).
+  Proof.
+    destruct (to_bv xbv1) as [bv1|] eqn:Hbv1; [apply bv_xbv_inverse in Hbv1; crush|].
+    intros. exfalso.
+  
+    bitvector_erase. subst.
+    apply (f_equal RawXBV.to_bv) in H.
+    rewrite RawXBV.xbv_bv_inverse in H.
+    rewrite RawXBV.has_x_to_bv in Hbv1.
+  
+    clear wf2. revert bv1 bv2 H Hbv1.
+    induction bv0; intros; [crush|].
+    unfold RawXBV.to_bv in *. simpl in *.
+    autodestruct_eqn E.
+    eauto.
+  Qed.
+  
+  Lemma concat_from_bv_inv2 n1 n2 (xbv1 : xbv n1) (xbv2 : xbv n2) bv :
+    concat xbv1 xbv2 = from_bv bv ->
+    (exists bv2, xbv2 = from_bv bv2).
+  Proof.
+    destruct (to_bv xbv2) as [bv2|] eqn:Hbv2; [apply bv_xbv_inverse in Hbv2; crush|].
+    intros. exfalso.
+  
+    bitvector_erase. subst.
+    apply (f_equal RawXBV.to_bv) in H.
+    rewrite RawXBV.xbv_bv_inverse in H.
+    rewrite RawXBV.has_x_to_bv in Hbv2.
+  
+    clear wf2. revert bv1 bv2 H Hbv2.
+    induction bv0; intros; [crush|].
+    unfold RawXBV.to_bv in *. simpl in *.
+    autodestruct_eqn E.
+    eauto.
+  Qed.
+  
+  Lemma concat_to_bv_none1 n1 n2 (xbv1 : xbv n1) (xbv2 : xbv n2) :
+    to_bv xbv1 = None ->
+    to_bv (concat xbv1 xbv2) = None.
+  Proof.
+    intros.
+    destruct (to_bv (concat xbv1 xbv2)) eqn:E; [exfalso|reflexivity].
+    apply bv_xbv_inverse in E. symmetry in E.
+    apply concat_from_bv_inv1 in E. destruct E. subst.
+    rewrite xbv_bv_inverse in H. discriminate.
+  Qed.
+  
+  Lemma concat_to_bv_none2 n1 n2 (xbv1 : xbv n1) (xbv2 : xbv n2) :
+    to_bv xbv2 = None ->
+    to_bv (concat xbv1 xbv2) = None.
+  Proof.
+    intros.
+    destruct (to_bv (concat xbv1 xbv2)) eqn:E; [exfalso|reflexivity].
+    apply bv_xbv_inverse in E. symmetry in E.
+    apply concat_from_bv_inv2 in E. destruct E. subst.
+    rewrite xbv_bv_inverse in H. discriminate.
+  Qed.
+  
+  Lemma extend_to_N w1 w2 (xbv : xbv w1) val :
+    to_N xbv = Some val ->
+    to_N (concat (zeros w2) xbv) = Some val.
+  Proof.
+    unfold to_N. intros.
+    destruct (to_bv xbv) as [bv|] eqn:Hbv; [|discriminate].
+    apply bv_xbv_inverse in Hbv. inv H.
+    rewrite zeros_from_bv. rewrite concat_no_exes.
+    rewrite xbv_bv_inverse. simpl. f_equal.
+    apply BV.bv_zextn_to_N.
+  Qed.
+  
+  Lemma extend_to_N_none2 w1 w2 (xbv1 : xbv w1) (xbv2 : xbv w2) :
+    to_N xbv2 = None ->
+    to_N (concat xbv1 xbv2) = None.
+  Proof.
+    unfold to_N. intros.
+    destruct (to_bv xbv2) eqn:E; simpl in *; [discriminate|].
+    rewrite concat_to_bv_none2; crush.
+  Qed.
+  
+  Lemma extr_shr_extend_overshift w1 w2 (xbv : xbv w1) shamt  :
+    (shamt > w1)%N ->
+    extr (shr (concat (zeros w2) xbv) shamt) 0 w1 =
+    shr xbv shamt.
+  Proof.
+    intros. bitvector_erase.
+    destruct (dec (shamt >= w2 + w1))%N.
+    - subst.
+      rewrite ! RawXBV.shr_overshift by (autorewrite with xbv_size in *; crush).
+      autorewrite with xbv_size.
+      eapply RawXBV.extr_of_zeros. lia.
+    - subst.
+      rewrite ! RawXBV.shr_overshift with (xbv:=bv0) by (autorewrite with xbv_size; crush).
+      rewrite ! RawXBV.shr_as_concat.
+      rewrite ! N2Nat.id.
+      fold (RawXBV.size bv0) in *.
+      autorewrite with xbv_size.
+      rewrite RawXBV.extr_of_concat with (xbv_lo := bv0) by (autorewrite with xbv_size; lia).
+      destruct_mins.
+      erewrite RawXBV.extr_of_zeros by lia.
+      erewrite RawXBV.concat_assoc.
+      erewrite RawXBV.concat_zeros.
+      erewrite RawXBV.extr_empty with (xbv := bv0) by lia.
+      erewrite RawXBV.concat_empty2 by reflexivity.
+      erewrite RawXBV.extr_of_zeros; crush.
+  Qed.
+  
+  Lemma extr_shr_extend_no_overshift w1 w2 (xbv : xbv w1) shamt  :
+    (shamt <= w1)%N ->
+    extr (shr (concat (zeros w2) xbv) shamt) 0 w1 =
+    shr xbv shamt.
+  Proof.
+    intros.
+    bitvector_erase. subst.
+    rewrite ! RawXBV.shr_as_concat.
+    rewrite ! N2Nat.id.
+    fold (RawXBV.size bv0) in *.
+    autorewrite with xbv_size.
+    rewrite ! RawXBV.extr_of_concat by (autorewrite with xbv_size; lia).
+    rewrite RawXBV.extr_of_zeros by (autorewrite with xbv_size; lia).
+    rewrite RawXBV.extr_of_zeros by (autorewrite with xbv_size; lia).
+    rewrite RawXBV.extr_of_zeros by (autorewrite with xbv_size; lia).
+    rewrite RawXBV.concat_assoc.
+    rewrite RawXBV.concat_zeros.
+    rewrite RawXBV.extr_of_extr by (autorewrite with xbv_size; lia).
+    autorewrite with xbv_size.
+    f_equal; f_equal; lia.
+  Qed.
+  
+  Lemma extr_shr_extend w1 w2 (xbv : xbv w1) shamt  :
+    extr (shr (concat (zeros w2) xbv) shamt) 0 w1 =
+    shr xbv shamt.
+  Proof.
+    destruct (dec (shamt <= w1))%N.
+    - eapply extr_shr_extend_no_overshift. eassumption.
+    - eapply extr_shr_extend_overshift. lia.
+  Qed.
+  
+  Lemma extr_shl_extend_overshift w1 w2 (xbv : xbv w1) shamt  :
+    (shamt > w1)%N ->
+    extr (shl (concat (zeros w2) xbv) shamt) 0 w1 =
+    shl xbv shamt.
+  Proof.
+    intros. bitvector_erase.
+    destruct (dec (shamt >= w2 + w1))%N.
+    - subst.
+      rewrite ! RawXBV.shl_overshift by (autorewrite with xbv_size; crush).
+      autorewrite with xbv_size.
+      eapply RawXBV.extr_of_zeros. lia.
+    - subst.
+      rewrite ! RawXBV.shl_overshift with (xbv:=bv0) by (autorewrite with xbv_size; crush).
+      rewrite ! RawXBV.shl_as_concat.
+      rewrite ! N2Nat.id.
+      fold (RawXBV.size bv0) in *.
+      autorewrite with xbv_size.
+      rewrite RawXBV.extr_of_concat with (xbv_lo := bv0) by (autorewrite with xbv_size; lia).
+      rewrite RawXBV.extr_of_concat_lo by (autorewrite with xbv_size; crush).
+      apply RawXBV.extr_of_zeros. lia.
+  Qed.
+  
+  Lemma extr_shl_extend_no_overshift w1 w2 (xbv : xbv w1) shamt  :
+    (shamt <= w1)%N ->
+    extr (shl (concat (zeros w2) xbv) shamt) 0 w1 =
+    shl xbv shamt.
+  Proof.
+    intros.
+    bitvector_erase. subst.
+    rewrite ! RawXBV.shl_as_concat.
+    rewrite ! N2Nat.id.
+    fold (RawXBV.size bv0) in *.
+    autorewrite with xbv_size.
+    rewrite ! RawXBV.extr_of_concat by (autorewrite with xbv_size; lia).
+    rewrite ! RawXBV.extr_of_zeros by (autorewrite with xbv_size; lia).
+    rewrite RawXBV.extr_of_extr by (autorewrite with xbv_size; lia).
+    autorewrite with xbv_size.
+    f_equal.
+    - rewrite RawXBV.concat_empty1 by (autorewrite with xbv_size; lia).
+      f_equal; crush.
+    - f_equal. crush.
+  Qed.
+  
+  Lemma extr_shl_extend w1 w2 (xbv : xbv w1) shamt :
+    extr (shl (concat (zeros w2) xbv) shamt) 0 w1 =
+    shl xbv shamt.
+  Proof.
+    destruct (dec (shamt <= w1))%N.
+    - eapply extr_shl_extend_no_overshift. eassumption.
+    - eapply extr_shl_extend_overshift. lia.
+  Qed.
+  
+  Lemma extr_exes n1 n2 lo :
+    extr (exes n1) lo n2 = exes n2.
+  Proof.
+    bitvector_erase. repeat unfold RawXBV.extr.
+    rewrite RawXBV.exes_size.
+    autodestruct_eqn E; kill_bools; [|reflexivity].
+    unfold RawXBV.exes.
+  
+    N_to_nat.
+    remember (List.repeat X n1) as xs.	 
+    funelim (RawXBV.extract xs lo n2).
+    - destruct n1; [|crush].
+      replace j with 0; crush.
+    - destruct n1; crush.
+    - destruct n1; [crush|].
+      simpl in *. specialize (H n1). insterU H.
+      crush.
+    - destruct n1; [crush|].
+      simpl in *. specialize (H n1). insterU H.
+      crush.
+  Qed.
+
+  Definition bit_of_as_bv i w (bv : BV.bitvector w) :
+    i < N.to_nat w ->
+    bitOf i (from_bv bv) = RawXBV.bool_to_bit (BV.bitOf i bv).
+  Proof.
+    destruct bv as [bv bv_wf]. unfold RawBV.size in *.
+    unfold bitOf, RawXBV.bitOf, from_bv, RawXBV.from_bv, BV.bitOf, RawBV.bitOf;
+      simpl.
+    intros.
+    rewrite List.nth_indep with (d':=O)
+      by (rewrite List.length_map; lia).
+    replace O with (RawXBV.bool_to_bit false)
+      by reflexivity.
+    apply List.map_nth.
+  Qed.
 End XBV.
