vera/VerilogToSMT/Expressions.v
@@ -39,798 +39,6 @@ Import EqNotations.
 
 Local Open Scope list.
 
-Ltac bitvector_erase :=
-  repeat match goal with
-         | [ xbv : XBV.xbv _ |- _ ] => destruct xbv
-         | [ bv : BV.bitvector _ |- _ ] => destruct bv
-         | [ H : RawXBV.size ?xbv = 0%N |- _ ] =>
-	   destruct xbv; [|discriminate]; clear H; simpl in *
-         | [ H : XBV.to_bv _ = None |- _ ] => rewrite <- XBV.has_x_to_bv in H
-         | [ H : ?xbv1 = ?xbv2 |- _ ] =>
-	   match type of xbv1 with
-	   | XBV.xbv _ =>
-	     apply (f_equal XBV.bits) in H; simpl in H
-	   | BV.bitvector _ =>
-	     apply (f_equal BV.bits) in H; simpl in H
-           end
-         | [ |- ?xbv1 = ?xbv2] =>
-	   match type of xbv1 with
-	   | XBV.xbv _ => apply XBV.of_bits_equal; simpl
-	   | BV.bitvector _ => apply BV.of_bits_equal; simpl
-           end
-         | [ |- context[rew _ in _] ] => destruct_rew
-	 end;
-  unfold XBV.has_x, BV.to_N in *; simpl in *.
-
-Lemma Nat2N_inj_le : forall n m, (N.of_nat n <= N.of_nat m)%N <-> n <= m.
-Proof. lia. Qed.
-
-Lemma Nat2N_inj_lt : forall n m, (N.of_nat n < N.of_nat m)%N <-> n < m.
-Proof. lia. Qed.
-
-Lemma N2Nat_inj_le : forall n m, (N.to_nat n <= N.to_nat m) <-> (n <= m)%N.
-Proof. lia. Qed.
-
-Lemma N2Nat_inj_lt : forall n m, (N.to_nat n < N.to_nat m) <-> (n < m)%N.
-Proof. lia. Qed.
-
-Hint Rewrite <- Nat2N.inj_add Nat2N.inj_mul Nat2N.inj_sub Nat2N.inj_min Nat2N.inj_max : N_to_nat.
-Hint Rewrite N2Nat.id Nat2N.id : N_to_nat.
-
-Ltac N_to_nat :=
-  repeat match goal with
-         | [ x : N |- _ ] =>
-	 let Heqx := fresh "Heq" in
-	 let x_temp := fresh x in
-	 remember (N.to_nat x) as x_temp eqn:Heqx;
-	 apply (f_equal N.of_nat) in Heqx;
-	 rewrite N2Nat.id in Heqx;
-	 rewrite <- Heqx in *;
-	 clear x Heqx;
-	 rename x_temp into x
-	 end;
-  autorewrite with N_to_nat in *;
-  repeat match goal with
-         | [ H : (_ <= _)%N |- _ ] => apply Nat2N_inj_le in H
-         | [ H : (_ < _)%N |- _ ] => apply Nat2N_inj_lt in H
-         | [ |- (_ <= _)%N ] => apply N2Nat_inj_le
-         | [ |- (_ < _)%N ] => apply N2Nat_inj_lt
-	 | _ => progress (autorewrite with N_to_nat in *)
-  end.
-
-Ltac destruct_mins := 
-    repeat match goal with
-           | [ |- context[N.min ?l ?r] ] =>
-	     let Heqmin := fresh "Heqmin" in (
-	       destruct (N.min_spec l r) as [[? Heqmin]|[? Heqmin]];
-	       rewrite Heqmin in *;
-	       clear Heqmin;
-	       try lia
-	     )
-           | [ H : context[N.min ?l ?r] |- _ ] =>
-	     let Heqmin := fresh "Heqmin" in (
-	       destruct (N.min_spec l r) as [[? Heqmin]|[? Heqmin]];
-	       rewrite Heqmin in *;
-	       clear Heqmin;
-	       try lia
-	     )
-           | [ |- context[Nat.min ?l ?r] ] =>
-	     let Heqmin := fresh "Heqmin" in (
-	       destruct (Nat.min_spec l r) as [[? Heqmin]|[? Heqmin]];
-	       rewrite Heqmin in *;
-	       clear Heqmin;
-	       try lia
-	     )
-           | [ H : context[Nat.min ?l ?r] |- _ ] =>
-	     let Heqmin := fresh "Heqmin" in (
-	       destruct (Nat.min_spec l r) as [[? Heqmin]|[? Heqmin]];
-	       rewrite Heqmin in *;
-	       clear Heqmin;
-	       try lia
-	     )
-	   end.
-
-Lemma fold_size bv : N.of_nat (List.length bv) = RawXBV.size bv.
-Proof. reflexivity. Qed.
-
-Lemma removelast_cons_size b bs : RawXBV.size (List.removelast (b :: bs)) = RawXBV.size bs.
-Proof. unfold RawXBV.size. now rewrite removelast_cons_length. Qed.
-
-Hint Rewrite
-  fold_size
-  @RawXBV.zeros_size @RawXBV.exes_size @RawXBV.ones_size
-  @RawXBV.concat_size @RawXBV.extr_width
-  @RawXBV.extract_width @RawXBV.extract_size
-  Nat2N.id N2Nat.id Nat2N.inj_min
-  @removelast_cons_length removelast_cons_size
-  : xbv_size.
-
-Hint Rewrite
-  N.leb_le N.leb_gt
-  Nat.leb_le Nat.leb_gt
-  : kill_bools.
-
-Ltac kill_bools := autorewrite with kill_bools in *.
-
-Program Definition empty : XBV.xbv 0 := {| XBV.bv := [] |}.
-
-Lemma xbv_zero_empty (xbv : XBV.xbv 0) : xbv = empty.
-Proof. bitvector_erase. reflexivity. Qed.
-
-Lemma raw_xbv_extract_full w (xbv : RawXBV.xbv) :
-  w = N.to_nat (RawXBV.size xbv) ->
-  RawXBV.extract xbv 0 w = xbv.
-Proof.
-  intros.
-  subst. unfold RawXBV.size. rewrite Nat2N.id.
-  funelim (RawXBV.extract xbv 0 (List.length xbv)); crush.
-Qed.
-
-Lemma raw_xbv_extract_empty lo sz (xbv : RawXBV.xbv) :
-  sz = 0 ->
-  RawXBV.extract xbv lo sz = [].
-Proof.
-  intros. subst.
-  funelim (RawXBV.extract xbv lo 0); crush.
-Qed.
-
-Lemma raw_xbv_extr_empty lo sz (xbv : RawXBV.xbv) :
-  (sz = 0)%N ->
-  RawXBV.extr xbv lo sz = [].
-Proof.
-  intros. subst. unfold RawXBV.extr.
-  rewrite raw_xbv_extract_empty by lia.
-  unfold RawXBV.exes; simpl. crush.
-Qed.
-
-Lemma xbv_extr_full w (xbv : XBV.xbv w) :
-  XBV.extr xbv 0 w = xbv.
-Proof.
-  bitvector_erase. subst.
-  unfold RawXBV.extr. unfold RawXBV.size. autodestruct_eqn E; [|crush].
-  rewrite Nat2N.id. simpl. clear E.
-  funelim (RawXBV.extract bv 0 (List.length bv)); crush.
-Qed.
-
-Lemma raw_xbv_concat_empty1 (xbv1 xbv2 : RawXBV.xbv) :
-  (RawXBV.size xbv1 = 0)%N ->
-  RawXBV.concat xbv1 xbv2 = xbv2.
-Proof. intros. unfold RawXBV.concat. destruct xbv1; [|crush]. now rewrite List.app_nil_r. Qed.
-
-Lemma raw_xbv_concat_empty2 (xbv1 xbv2 : RawXBV.xbv) :
-  (RawXBV.size xbv2 = 0)%N ->
-  RawXBV.concat xbv1 xbv2 = xbv1.
-Proof. intros. unfold RawXBV.concat. destruct xbv2; crush. Qed.
-
-Lemma xbv_concat_empty1 w (xbv1 : XBV.xbv 0) (xbv2 : XBV.xbv w) :
-  XBV.concat xbv1 xbv2 = xbv2.
-Proof. bitvector_erase. unfold RawXBV.concat. now rewrite List.app_nil_r. Qed.
-
-(* Types don't match for this one (w + 0 is not definitionally equal to w) *)
-(* Lemma xbv_concat_empty2 w (xbv1 : XBV.xbv w) (xbv2 : XBV.xbv 0) :
- *   XBV.concat xbv1 xbv2 = xbv1.
- * Proof. bitvector_erase. induction bv. crush. Qed. *)
-
-Lemma zeros_from_bv n : XBV.zeros n = XBV.from_bv (BV.zeros n).
-Proof.
-  apply XBV.of_bits_equal. simpl. unfold RawBV.zeros, RawXBV.zeros.
-  induction n using N.peano_ind; simpl.
-  - reflexivity.
-  - rewrite N2Nat.inj_succ. simpl. crush.
-Qed.
-
-Lemma concat_from_bv n1 n2 bv1 bv2 :
-  XBV.concat (XBV.from_bv (n:=n1) bv1) (XBV.from_bv (n:=n2) bv2) = XBV.from_bv (BV.bv_concat bv1 bv2).
-Proof.
-  apply XBV.of_bits_equal. simpl.
-  destruct bv1 as [bv1 wf1], bv2 as [bv2 wf2]. subst. simpl.
-  revert bv1.
-  induction bv2; crush.
-Qed.
-
-Lemma concat_from_bv_inv1 n1 n2 (xbv1 : XBV.xbv n1) (xbv2 : XBV.xbv n2) bv :
-  XBV.concat xbv1 xbv2 = XBV.from_bv bv ->
-  (exists bv1, xbv1 = XBV.from_bv bv1).
-Proof.
-  destruct (XBV.to_bv xbv1) as [bv1|] eqn:Hbv1; [apply XBV.bv_xbv_inverse in Hbv1; crush|].
-  intros. exfalso.
-
-  bitvector_erase. subst.
-  apply (f_equal RawXBV.to_bv) in H.
-  rewrite RawXBV.xbv_bv_inverse in H.
-  rewrite RawXBV.has_x_to_bv in Hbv1.
-
-  clear wf1. revert bv bv1 H Hbv1.
-  induction bv0; intros; [crush|].
-  unfold RawXBV.to_bv in *. simpl in *.
-  autodestruct_eqn E.
-  eauto.
-Qed.
-
-Lemma concat_from_bv_inv2 n1 n2 (xbv1 : XBV.xbv n1) (xbv2 : XBV.xbv n2) bv :
-  XBV.concat xbv1 xbv2 = XBV.from_bv bv ->
-  (exists bv2, xbv2 = XBV.from_bv bv2).
-Proof.
-  destruct (XBV.to_bv xbv2) as [bv2|] eqn:Hbv2; [apply XBV.bv_xbv_inverse in Hbv2; crush|].
-  intros. exfalso.
-
-  bitvector_erase. subst.
-  apply (f_equal RawXBV.to_bv) in H.
-  rewrite RawXBV.xbv_bv_inverse in H.
-  rewrite RawXBV.has_x_to_bv in Hbv2.
-
-  clear wf1. revert bv bv1 H Hbv2.
-  induction bv0; intros; [crush|].
-  unfold RawXBV.to_bv in *. simpl in *.
-  autodestruct_eqn E.
-  eauto.
-Qed.
-
-Lemma concat_to_bv_none1 n1 n2 (xbv1 : XBV.xbv n1) (xbv2 : XBV.xbv n2) :
-  XBV.to_bv xbv1 = None ->
-  XBV.to_bv (XBV.concat xbv1 xbv2) = None.
-Proof.
-  intros.
-  destruct (XBV.to_bv (XBV.concat xbv1 xbv2)) eqn:E; [exfalso|reflexivity].
-  apply XBV.bv_xbv_inverse in E. symmetry in E.
-  apply concat_from_bv_inv1 in E. destruct E. subst.
-  rewrite XBV.xbv_bv_inverse in H. discriminate.
-Qed.
-
-Lemma concat_to_bv_none2 n1 n2 (xbv1 : XBV.xbv n1) (xbv2 : XBV.xbv n2) :
-  XBV.to_bv xbv2 = None ->
-  XBV.to_bv (XBV.concat xbv1 xbv2) = None.
-Proof.
-  intros.
-  destruct (XBV.to_bv (XBV.concat xbv1 xbv2)) eqn:E; [exfalso|reflexivity].
-  apply XBV.bv_xbv_inverse in E. symmetry in E.
-  apply concat_from_bv_inv2 in E. destruct E. subst.
-  rewrite XBV.xbv_bv_inverse in H. discriminate.
-Qed.
-
-Lemma extend_to_N w1 w2 (xbv : XBV.xbv w1) val :
-  XBV.to_N xbv = Some val ->
-  XBV.to_N (XBV.concat (XBV.zeros w2) xbv) = Some val.
-Proof.
-  unfold XBV.to_N. intros.
-  destruct (XBV.to_bv xbv) as [bv|] eqn:Hbv; [|discriminate].
-  apply XBV.bv_xbv_inverse in Hbv. inv H.
-  rewrite zeros_from_bv. rewrite concat_from_bv.
-  rewrite XBV.xbv_bv_inverse. simpl. f_equal.
-  apply BV.bv_zextn_to_N.
-Qed.
-
-Lemma extend_to_N_none2 w1 w2 (xbv1 : XBV.xbv w1) (xbv2 : XBV.xbv w2) :
-  XBV.to_N xbv2 = None ->
-  XBV.to_N (XBV.concat xbv1 xbv2) = None.
-Proof.
-  unfold XBV.to_N. intros.
-  destruct (XBV.to_bv xbv2) eqn:E; simpl in *; [discriminate|].
-  rewrite concat_to_bv_none2; crush.
-Qed.
-
-Lemma shr_as_concat_gt (n : nat) (xbv : RawXBV.xbv) :
-  (List.length xbv < n) ->
-  RawXBV.shr xbv n = RawXBV.zeros (RawXBV.size xbv).
-Proof.
-  funelim (RawXBV.shr xbv n); intros; unfold RawXBV.zeros; simpl in *.
-  - destruct bv; crush.
-  - reflexivity.
-  - insterU H.
-    unfold RawXBV.zeros in *.
-    rewrite Pnat.SuccNat2Pos.id_succ.
-    rewrite Nat2N.id in *.
-    simpl. rewrite H.
-    clear Heqcall H0 H.
-    induction (List.length bs); crush.
-Qed.
-
-Lemma shr_as_concat_le (n : nat) (xbv : RawXBV.xbv) :
-  (n <= List.length xbv) ->
-  RawXBV.shr xbv n =
-    RawXBV.concat
-      (RawXBV.zeros (N.of_nat n))
-      (RawXBV.extr xbv (N.of_nat n) (RawXBV.size xbv - N.of_nat n)).
-Proof.
-  unfold RawXBV.zeros, RawXBV.concat, RawXBV.extr, RawXBV.size.
-  simpl. rewrite Nat2N.id.
-  intros.
-  autodestruct_eqn E; kill_bools; try lia.
-  funelim (RawXBV.shr xbv n); [idtac|crush|idtac].
-  + simpl in *.
-    rewrite raw_xbv_extract_full. 
-    * now rewrite List.app_nil_r. 
-    * unfold RawXBV.size. lia.
-  + insterU H. simp extract.
-    rewrite H. clear H.
-    rewrite ! N2Nat.inj_sub, ! Nat2N.id.
-    simpl.
-    rewrite <- List.app_assoc. f_equal.
-    clear E H0 Heqcall. induction n; crush.
-Qed.
-
-Lemma shr_as_concat (n : nat) (xbv : RawXBV.xbv) :
-  RawXBV.shr xbv n =
-    RawXBV.concat
-      (RawXBV.zeros (N.of_nat (min (List.length xbv) n)))
-      (RawXBV.extr xbv (N.of_nat n) (RawXBV.size xbv - N.of_nat n)).
-Proof.
-  destruct (Nat.leb n (List.length xbv)) eqn:E; kill_bools.
-  - rewrite Nat.min_r by lia.
-    apply shr_as_concat_le. lia.
-  - rewrite Nat.min_l by lia.
-    rewrite shr_as_concat_gt by lia.
-    unfold RawXBV.extr.
-    autodestruct_eqn Hcmp; [crush|clear Hcmp].
-    rewrite raw_xbv_concat_empty2. reflexivity.
-    rewrite RawXBV.exes_size. unfold RawXBV.size. lia.
-Qed.
-
-Lemma shl_as_concat_gt (n : nat) (xbv : RawXBV.xbv) :
-  (List.length xbv < n) ->
-  RawXBV.shl xbv n = RawXBV.zeros (RawXBV.size xbv).
-Proof.
-  funelim (RawXBV.shl xbv n); intros.
-  - destruct bv; crush.
-  - reflexivity.
-  - insterU H.
-    autorewrite with xbv_size in *.
-    unfold RawXBV.size, RawXBV.zeros in *. cbn [List.length] in *.
-    erewrite H by lia. N_to_nat. reflexivity.
-Qed.
-
-Lemma rawxbv_extract_remove_last n l:
-  n < List.length l ->
-  RawXBV.extract (List.removelast l) 0 n = RawXBV.extract l 0 n.
-Proof.
-  revert n.
-  induction l; intros.
-  - destruct n; [|crush]. reflexivity.
-  - simpl in H.
-    destruct n; [rewrite ! raw_xbv_extract_empty; crush|].
-    simp extract. destruct l; [crush|].
-    simpl. simp extract.
-    f_equal. apply IHl. lia.
-Qed.
-
-Lemma shl_as_concat_le (n : nat) (xbv : RawXBV.xbv) :
-  (n <= List.length xbv) ->
-  RawXBV.shl xbv n =
-    RawXBV.concat
-      (RawXBV.extr xbv 0 (RawXBV.size xbv - N.of_nat n))
-      (RawXBV.zeros (N.of_nat n)).
-Proof.
-  unfold RawXBV.zeros, RawXBV.concat, RawXBV.extr, RawXBV.size.
-  simpl. rewrite Nat2N.id.
-  intros.
-  autodestruct_eqn E; kill_bools; N_to_nat; try lia.
-  funelim (RawXBV.shl xbv n); [idtac|crush|idtac].
-  + simpl in *.
-    rewrite raw_xbv_extract_full. 
-    * reflexivity.
-    * unfold RawXBV.size. lia.
-  + insterU H. simp extract.
-    rewrite H by (autorewrite with xbv_size in *; crush).
-    clear H. cbn [List.repeat List.app]. do 2 f_equal.
-    autorewrite with xbv_size.
-    apply rawxbv_extract_remove_last.
-    lia.
-Qed.
-
-(* TO BE UPDATED *)
-Lemma shl_as_concat (n : nat) (xbv : RawXBV.xbv) :
-  RawXBV.shl xbv n =
-    RawXBV.concat
-      (RawXBV.extr xbv 0 (RawXBV.size xbv - N.of_nat n))
-      (RawXBV.zeros (N.of_nat (min (List.length xbv) n)))
-      .
-Proof.
-  destruct (Nat.leb n (List.length xbv)) eqn:E; kill_bools.
-  - rewrite Nat.min_r by lia.
-    apply shl_as_concat_le. lia.
-  - rewrite Nat.min_l by lia.
-    rewrite shl_as_concat_gt by lia.
-    unfold RawXBV.extr.
-    autodestruct_eqn Hcmp; kill_bools; [|crush].
-    rewrite raw_xbv_concat_empty1. reflexivity.
-    autorewrite with xbv_size. unfold RawXBV.size in *. lia.
-Qed.
-
-Lemma extract_width x i j :
-  (j + i <= List.length x) ->
-  List.length (RawXBV.extract x i j) = (Nat.min j (List.length x - i)).
-Proof.
-  funelim (RawXBV.extract x i j);
-    simp extract; simpl in *; try crush.
-Qed.
-
-Lemma rawxbv_extr_of_concat_lo xbv_hi xbv_lo lo sz :
-  (lo <= RawXBV.size xbv_lo)%N ->
-  (lo + sz <= RawXBV.size xbv_lo)%N ->
-  RawXBV.extr (RawXBV.concat xbv_hi xbv_lo) lo sz = RawXBV.extr xbv_lo lo sz.
-Proof.
-  intros Hlo Hhi.
-  unfold RawXBV.extr.
-  autodestruct_eqn E; kill_bools;
-    autorewrite with xbv_size in *;
-    try lia; [idtac].
-  clear E E0.
-  N_to_nat. unfold RawXBV.concat.
-  funelim (RawXBV.extract xbv_lo lo sz).
-  - simpl in *.
-    replace i with 0 by lia.
-    replace j with 0 by lia. 
-    destruct xbv_hi; simp extract; reflexivity.
-  - simpl in *. simp extract. reflexivity.
-  - simpl in *. simp extract.
-    erewrite H; try crush.
-  - simpl in *. simp extract. eapply H; lia.
-Qed.
-
-Lemma rawxbv_extr_of_concat_hi xbv_hi xbv_lo lo sz :
-  (RawXBV.size xbv_lo <= lo)%N ->
-  (lo + sz <= RawXBV.size xbv_lo + RawXBV.size xbv_hi)%N ->
-  RawXBV.extr (RawXBV.concat xbv_hi xbv_lo) lo sz =
-    RawXBV.extr xbv_hi (lo - RawXBV.size xbv_lo) sz.
-Proof.
-  intros Hlo Hhi.
-  unfold RawXBV.extr.
-  autodestruct_eqn E; kill_bools;
-    autorewrite with xbv_size in *;
-    try lia; [idtac].
-  clear E E0.
-  unfold RawXBV.size, RawXBV.concat in *.
-  N_to_nat.
-  funelim (RawXBV.extract (xbv_lo ++ xbv_hi) lo sz); intros.
-  - symmetry in H. apply List.app_eq_nil in H.
-    destruct H. subst. simp extract. reflexivity.
-  - destruct xbv_lo; [|crush]. simpl.
-    destruct xbv_hi; now simp extract.
-  - destruct xbv_lo; [|crush]. simpl in *. subst.
-    simp extract. reflexivity.
-  - destruct xbv_lo; simpl in *.
-    + subst. simp extract. reflexivity.
-    + inv H0. eapply H; crush.
-Qed.
-
-Lemma rawxbv_extr_of_concat_mid xbv_hi xbv_lo lo sz :
-  (lo <= RawXBV.size xbv_lo)%N ->
-  (RawXBV.size xbv_lo <= lo + sz)%N ->
-  (lo + sz <= RawXBV.size xbv_lo + RawXBV.size xbv_hi)%N ->
-  RawXBV.extr (RawXBV.concat xbv_hi xbv_lo) lo sz =
-    RawXBV.concat
-      (RawXBV.extr xbv_hi (lo - RawXBV.size xbv_lo)%N (sz - (RawXBV.size xbv_lo - lo))%N)
-      (RawXBV.extr xbv_lo lo (RawXBV.size xbv_lo - lo)%N).
-Proof.
-  intros Hlo Hmid Hhi.
-  unfold RawXBV.extr.
-  autodestruct_eqn E; kill_bools;
-    autorewrite with xbv_size in *;
-    try lia; [idtac].
-  clear E E0 E1.
-  unfold RawXBV.size, RawXBV.concat in *.
-  N_to_nat.
-  funelim (RawXBV.extract (xbv_lo ++ xbv_hi) lo sz); intros.
-  - symmetry in H. apply List.app_eq_nil in H.
-    destruct H. subst. simp extract. reflexivity.
-  - destruct xbv_lo; [|crush]. simpl.
-    destruct xbv_hi; now simp extract.
-  - destruct xbv_lo.
-    + simpl in *. subst. simpl. simp extract. simpl.
-      repeat f_equal.
-    + simpl in *. inv H0. simp extract. simpl. f_equal.
-      erewrite H by crush.
-      repeat f_equal; try crush.
-  - destruct xbv_lo; [crush|]. simpl in *. simp extract.
-    inv H0. erewrite H by crush.
-    f_equal.
-Qed.
-
-Lemma rawxbv_extr_of_concat xbv_hi xbv_lo lo sz :
-  (lo + sz <= RawXBV.size xbv_hi + RawXBV.size xbv_lo)%N ->
-  RawXBV.extr (RawXBV.concat xbv_hi xbv_lo) lo sz =
-    RawXBV.concat
-      (RawXBV.extr xbv_hi (lo - RawXBV.size xbv_lo) (sz - (RawXBV.size xbv_lo - lo)))%N
-      (RawXBV.extr xbv_lo lo (N.min sz (RawXBV.size xbv_lo - lo)))%N.
-Proof.
-  intros.
-  destruct (dec (RawXBV.size xbv_lo <= lo)%N);
-    destruct (dec (lo + sz < RawXBV.size xbv_lo))%N; try lia.
-  - replace (N.min sz (RawXBV.size xbv_lo - lo)) with (RawXBV.size xbv_lo - lo)%N by lia.
-    replace (RawXBV.size xbv_lo - lo)%N with 0%N by lia.
-    erewrite rawxbv_extr_of_concat_hi by lia.
-    rewrite raw_xbv_concat_empty2 by (autorewrite with xbv_size; lia).
-    f_equal. lia.
-  - replace (N.min sz (RawXBV.size xbv_lo - lo)) with sz by lia.
-    replace (sz - (RawXBV.size xbv_lo - lo))%N with 0%N by lia.
-    erewrite rawxbv_extr_of_concat_lo by lia.
-    rewrite raw_xbv_concat_empty1 by (autorewrite with xbv_size; lia).
-    reflexivity.
-  - replace (N.min sz (RawXBV.size xbv_lo - lo)) with (RawXBV.size xbv_lo - lo)%N by lia.
-    eapply rawxbv_extr_of_concat_mid; lia.
-Qed.
-
-Lemma rawxbv_extr_of_zeros w lo sz :
-  (lo + sz <= w)%N ->
-  RawXBV.extr (RawXBV.zeros w) lo sz = RawXBV.zeros sz.
-Proof.
-  intros. unfold RawXBV.extr.
-  autorewrite with xbv_size. autodestruct_eqn E; [clear E|crush].
-  unfold RawXBV.zeros.
-  N_to_nat.
-  revert lo sz H.
-  induction w; intros; simpl; simp extract.
-  - replace sz with 0; crush.
-  - destruct lo, sz; simpl; simp extract.
-    + reflexivity.
-    + erewrite IHw; crush.
-    + erewrite IHw; crush.
-    + erewrite IHw; crush.
-Qed.
-
-Lemma rawxbv_extr_of_extr lo1 lo2 sz1 sz2 xbv :
-  (lo1 + sz1 <= RawXBV.size xbv)%N ->
-  (lo2 + sz2 <= sz1)%N ->
-  RawXBV.extr (RawXBV.extr xbv lo1 sz1) lo2 sz2 = RawXBV.extr xbv (lo1 + lo2) sz2.
-Proof.
-  intros H0 H1.
-  unfold RawXBV.extr.
-  autodestruct_eqn E;
-    autorewrite with xbv_size kill_bools in *;
-    try crush; N_to_nat.
-  clear E E0 E1.
-  revert sz1 H0 H1.
-  funelim (RawXBV.extract xbv (lo1 + lo2) sz2).
-  - intros. simp extract. reflexivity.
-  - intros.
-    replace lo2 with 0 in * by lia.
-    destruct (RawXBV.extract (bx :: x') lo1 sz1); simp extract; reflexivity.
-  - intros. simpl in *. clear Heqcall.
-    replace lo1 with 0 in * by crush.
-    replace lo2 with 0 in * by crush.
-    destruct sz1; [lia|].
-    simp extract.
-    erewrite H; crush.
-  - intros. simpl in *. clear Heqcall.
-    destruct lo1, sz1;
-      simpl in *; subst; simp extract.
-    + lia.
-    + erewrite H; crush.
-    + erewrite H; crush.
-    + erewrite H; crush.
-Qed.
-
-Lemma concat_assoc x1 x2 x3 :
-  RawXBV.concat x1 (RawXBV.concat x2 x3) = RawXBV.concat (RawXBV.concat x1 x2) x3.
-Proof. unfold RawXBV.concat. now rewrite List.app_assoc. Qed.
-
-Lemma concat_zeros w1 w2 :
-  RawXBV.concat (RawXBV.zeros w1) (RawXBV.zeros w2) = RawXBV.zeros (w1 + w2).
-Proof.
-  unfold RawXBV.zeros, RawXBV.concat.
-  rewrite <- List.repeat_app. f_equal. lia.
-Qed.
-
-Lemma raw_xbv_shr_overshift xbv shamt :
-  (N.of_nat shamt >= RawXBV.size xbv)%N ->
-  RawXBV.shr xbv shamt = RawXBV.zeros (RawXBV.size xbv).
-Proof.
-  intros.
-  unfold RawXBV.size, RawXBV.zeros in *.
-  N_to_nat.
-  funelim (RawXBV.shr xbv shamt).
-  - destruct bv; crush.
-  - reflexivity.
-  - cbn [List.length] in *.
-    rewrite H by lia. clear H H0 Heqcall.
-    induction (List.length bs); crush.
-Qed.
-
-Lemma xbv_shr_overshift w (xbv : XBV.xbv w) shamt :
-  (shamt >= w)%N ->
-  XBV.shr xbv shamt = XBV.zeros w.
-Proof.
-  intros.
-  bitvector_erase. subst.
-  erewrite raw_xbv_shr_overshift; unfold RawXBV.size in *; crush.
-Qed.
-
-Lemma extr_shr_extend_overshift w1 w2 (xbv : XBV.xbv w1) shamt  :
-  (shamt > w1)%N ->
-  XBV.extr (XBV.shr (XBV.concat (XBV.zeros w2) xbv) shamt) 0 w1 =
-  XBV.shr xbv shamt.
-Proof.
-  intros. bitvector_erase.
-  destruct (dec (shamt >= w2 + w1))%N.
-  - subst.
-    rewrite ! raw_xbv_shr_overshift by (autorewrite with xbv_size; crush).
-    autorewrite with xbv_size.
-    eapply rawxbv_extr_of_zeros. lia.
-  - subst.
-    rewrite ! raw_xbv_shr_overshift with (xbv:=bv) by (autorewrite with xbv_size; crush).
-    rewrite ! shr_as_concat.
-    rewrite ! N2Nat.id.
-    fold (RawXBV.size bv) in *.
-    autorewrite with xbv_size.
-    rewrite rawxbv_extr_of_concat with (xbv_lo := bv) by (autorewrite with xbv_size; lia).
-    destruct_mins.
-    erewrite rawxbv_extr_of_zeros by lia.
-    erewrite concat_assoc.
-    erewrite concat_zeros.
-    erewrite raw_xbv_extr_empty with (xbv := bv) by lia.
-    erewrite raw_xbv_concat_empty2 by reflexivity.
-    erewrite rawxbv_extr_of_zeros; crush.
-Qed.
-
-Lemma extr_shr_extend_no_overshift w1 w2 (xbv : XBV.xbv w1) shamt  :
-  (shamt <= w1)%N ->
-  XBV.extr (XBV.shr (XBV.concat (XBV.zeros w2) xbv) shamt) 0 w1 =
-  XBV.shr xbv shamt.
-Proof.
-  intros.
-  bitvector_erase. subst.
-  rewrite ! shr_as_concat.
-  rewrite ! N2Nat.id.
-  fold (RawXBV.size bv) in *.
-  autorewrite with xbv_size.
-  rewrite ! rawxbv_extr_of_concat by (autorewrite with xbv_size; lia).
-  rewrite rawxbv_extr_of_zeros by (autorewrite with xbv_size; lia).
-  rewrite rawxbv_extr_of_zeros by (autorewrite with xbv_size; lia).
-  rewrite rawxbv_extr_of_zeros by (autorewrite with xbv_size; lia).
-  rewrite concat_assoc.
-  rewrite concat_zeros.
-  rewrite rawxbv_extr_of_extr by (autorewrite with xbv_size; lia).
-  autorewrite with xbv_size.
-  f_equal; f_equal; lia.
-Qed.
-
-Lemma extr_shr_extend w1 w2 (xbv : XBV.xbv w1) shamt  :
-  XBV.extr (XBV.shr (XBV.concat (XBV.zeros w2) xbv) shamt) 0 w1 =
-  XBV.shr xbv shamt.
-Proof.
-  destruct (dec (shamt <= w1))%N.
-  - eapply extr_shr_extend_no_overshift. eassumption.
-  - eapply extr_shr_extend_overshift. lia.
-Qed.
-
-
-Lemma raw_xbv_shl_overshift xbv shamt :
-  (N.of_nat shamt >= RawXBV.size xbv)%N ->
-  RawXBV.shl xbv shamt = RawXBV.zeros (RawXBV.size xbv).
-Proof.
-  intros.
-  unfold RawXBV.size, RawXBV.zeros in *.
-  N_to_nat.
-  funelim (RawXBV.shl xbv shamt).
-  - destruct bv; crush.
-  - reflexivity.
-  - cbn [List.length] in *.
-    erewrite H by (autorewrite with xbv_size; crush).
-    autorewrite with xbv_size.
-    crush.
-Qed.
-
-Lemma xbv_shl_overshift w (xbv : XBV.xbv w) shamt :
-  (shamt >= w)%N ->
-  XBV.shl xbv shamt = XBV.zeros w.
-Proof.
-  intros.
-  bitvector_erase. subst.
-  erewrite raw_xbv_shl_overshift; unfold RawXBV.size in *; crush.
-Qed.
-
-Lemma extr_shl_extend_overshift w1 w2 (xbv : XBV.xbv w1) shamt  :
-  (shamt > w1)%N ->
-  XBV.extr (XBV.shl (XBV.concat (XBV.zeros w2) xbv) shamt) 0 w1 =
-  XBV.shl xbv shamt.
-Proof.
-  intros. bitvector_erase.
-  destruct (dec (shamt >= w2 + w1))%N.
-  - subst.
-    rewrite ! raw_xbv_shl_overshift by (autorewrite with xbv_size; crush).
-    autorewrite with xbv_size.
-    eapply rawxbv_extr_of_zeros. lia.
-  - subst.
-    rewrite ! raw_xbv_shl_overshift with (xbv:=bv) by (autorewrite with xbv_size; crush).
-    rewrite ! shl_as_concat.
-    rewrite ! N2Nat.id.
-    fold (RawXBV.size bv) in *.
-    autorewrite with xbv_size.
-    rewrite rawxbv_extr_of_concat with (xbv_lo := bv) by (autorewrite with xbv_size; lia).
-    rewrite rawxbv_extr_of_concat_lo by (autorewrite with xbv_size; crush).
-    apply rawxbv_extr_of_zeros. lia.
-Qed.
-
-Lemma extr_shl_extend_no_overshift w1 w2 (xbv : XBV.xbv w1) shamt  :
-  (shamt <= w1)%N ->
-  XBV.extr (XBV.shl (XBV.concat (XBV.zeros w2) xbv) shamt) 0 w1 =
-  XBV.shl xbv shamt.
-Proof.
-  intros.
-  bitvector_erase. subst.
-  rewrite ! shl_as_concat.
-  rewrite ! N2Nat.id.
-  fold (RawXBV.size bv) in *.
-  autorewrite with xbv_size.
-  rewrite ! rawxbv_extr_of_concat by (autorewrite with xbv_size; lia).
-  rewrite ! rawxbv_extr_of_zeros by (autorewrite with xbv_size; lia).
-  rewrite rawxbv_extr_of_extr by (autorewrite with xbv_size; lia).
-  autorewrite with xbv_size.
-  f_equal.
-  - rewrite raw_xbv_concat_empty1 by (autorewrite with xbv_size; lia).
-    f_equal; crush.
-  - f_equal. crush.
-Qed.
-
-Lemma extr_shl_extend w1 w2 (xbv : XBV.xbv w1) shamt :
-  XBV.extr (XBV.shl (XBV.concat (XBV.zeros w2) xbv) shamt) 0 w1 =
-  XBV.shl xbv shamt.
-Proof.
-  destruct (dec (shamt <= w1))%N.
-  - eapply extr_shl_extend_no_overshift. eassumption.
-  - eapply extr_shl_extend_overshift. lia.
-Qed.
-
-Lemma extr_exes n1 n2 lo :
-  XBV.extr (XBV.exes n1) lo n2 = XBV.exes n2.
-Proof.
-  bitvector_erase. repeat unfold RawXBV.extr.
-  rewrite RawXBV.exes_size.
-  autodestruct_eqn E; kill_bools; [|reflexivity].
-  unfold RawXBV.exes.
-
-  N_to_nat.
-  remember (List.repeat X n1) as xs.	 
-  funelim (RawXBV.extract xs lo n2).
-  - destruct n1; [|crush].
-    replace j with 0; crush.
-  - destruct n1; crush.
-  - destruct n1; [crush|].
-    (* rewrite ! Nat2N.inj_succ in *. *)
-    simpl in *. specialize (H n1). insterU H.
-    crush.
-  - destruct n1; [crush|].
-    simpl in *. specialize (H n1). insterU H.
-    crush.
-Qed.
-
-(* Move me to bitvector *)
-Lemma bv_shr_swap_definition w lhs rhs :
-  BV.bv_shr (n:=w) lhs rhs = BV.shr lhs (BV.to_N rhs).
-Proof.
- bitvector_erase.
- unfold RawBV.bv_shr, RawBV.to_N in *.
- rewrite wf, wf0, N.eqb_refl, Nat2N.id in *.
- clear wf wf0.
- unfold RawBV.shr_be.
- rewrite RawBV.shr_be_nicify.
- generalize dependent (RawBV.list2nat_be bv).
- intros shamt. clear w bv.
- unfold RawBV.size in *.
- funelim (RawBV.shr bv0 shamt).
- - destruct bv; simp nice_nshr_be; reflexivity.
- - simp nice_nshr_be. crush.
- - simp nice_nshr_be. crush.
-Qed.
-
-Lemma bv_shl_swap_definition w lhs rhs :
-  BV.bv_shl (n:=w) lhs rhs = BV.shl lhs (BV.to_N rhs).
-Proof.
- bitvector_erase.
- unfold RawBV.bv_shl, RawBV.to_N in *.
- rewrite wf, wf0, N.eqb_refl, Nat2N.id in *.
- clear wf wf0.
- unfold RawBV.shl_be.
- rewrite RawBV.shl_be_nicify.
- generalize dependent (RawBV.list2nat_be bv).
- intros shamt. clear w bv.
- unfold RawBV.size in *.
- funelim (RawBV.shl bv0 shamt).
- - destruct bv; simp nice_nshl_be; reflexivity.
- - simp nice_nshl_be. crush.
- - simp nice_nshl_be. crush.
-Qed.
-
 Lemma bitwise_binop_no_exes (f_bit : bit -> bit -> bit) (f_bool : bool -> bool -> bool) :
   (forall (lb rb : bool), RawXBV.bool_to_bit (f_bool lb rb) = f_bit (RawXBV.bool_to_bit lb) (RawXBV.bool_to_bit rb)) ->
   forall n (l_xbv r_xbv : XBV.xbv n) (l_bv r_bv : BV.bitvector n),
@@ -898,95 +106,8 @@ Proof.
   reflexivity.
 Qed.
 
-Lemma xbv_concat_no_exes w1 w2 (bv1 : BV.bitvector w1) (bv2 : BV.bitvector w2) :
-  XBV.concat (XBV.from_bv bv1) (XBV.from_bv bv2) =
-    XBV.from_bv (BV.bv_concat bv1 bv2).
-Proof.
-  destruct bv1 as [bv1 wf1], bv2 as [bv2 wf2].
-  apply XBV.of_bits_equal. simpl.
-  unfold RawBV.bv_concat, RawXBV.from_bv.
-  rewrite List.map_app.
-  reflexivity.
-Qed.
-
-Lemma xbv_concat_to_bv w1 w2 (bv1 : BV.bitvector w1) (bv2 : BV.bitvector w2) :
-  XBV.to_bv (XBV.concat (XBV.from_bv bv1) (XBV.from_bv bv2)) =
-    Some (BV.bv_concat bv1 bv2).
-Proof.
-  rewrite xbv_concat_no_exes.
-  rewrite XBV.xbv_bv_inverse.
-  reflexivity.
-Qed.
-
-Lemma bv_extr_one_bit (n : N) w (bv : BV.bitvector w) :
-  (1 + n <= w)%N ->
-  BV.bv_extr n 1 bv = BV.of_bits [BV.bitOf (N.to_nat n) bv].
-Proof.
-  destruct bv as [bv wf].
-  subst. intros.
-  apply BV.of_bits_equal.
-  simpl.
-  unfold BV.bv_extr, RawBV.bv_extr, RawBV.size in *.
-  autodestruct_eqn E; try (rewrite N.ltb_lt in *; lia); clear E.
-  replace (N.to_nat (1 + n)) with (S (N.to_nat n)) by lia.
-  assert (S (N.to_nat n) <= List.length bv) as H' by lia. clear H. revert H'.
-  generalize (N.to_nat n). clear n. intros n H.
-  revert bv H.
-  induction n; intros.
-  { destruct bv; try crush.
-    destruct bv; crush.
-  }
-  destruct bv; try crush.
-  simpl.
-  rewrite IHn; crush.
-Qed.
-
-Definition bit_of_as_bv i w (bv : BV.bitvector w) :
-  i < N.to_nat w ->
-  XBV.bitOf i (XBV.from_bv bv) = RawXBV.bool_to_bit (BV.bitOf i bv).
-Proof.
-  destruct bv as [bv bv_wf]. unfold RawBV.size in *.
-  unfold XBV.bitOf, RawXBV.bitOf, XBV.from_bv, RawXBV.from_bv, BV.bitOf, RawBV.bitOf;
-    simpl.
-  intros.
-  rewrite List.nth_indep with (d':=O)
-    by (rewrite List.length_map; lia).
-  replace O with (RawXBV.bool_to_bit false)
-    by reflexivity.
-  apply List.map_nth.
-Qed.
-
 Definition select_bit_bv {w1 w2} (vec : BV.bitvector w1) (idx : BV.bitvector w2) : BV.bitvector 1 :=
   BV.of_bits [BV.bitOf (N.to_nat (BV.to_N idx)) vec].
-
-Lemma to_bv_some_raw_iff w (xbv : XBV.xbv w) (bv : BV.bitvector w) :
-  XBV.to_bv xbv = Some bv <-> RawXBV.to_bv (XBV.bits xbv) = Some (BV.bits bv).
-Proof.
-  (* This is disgusting (written while half asleep) plzfix *)
-  split; intros; simpl in *.
-  - apply XBV.bv_xbv_inverse in H. subst.
-    destruct bv as [bv bv_wf].
-    simpl. apply RawXBV.xbv_bv_inverse.
-  - apply RawXBV.bv_xbv_inverse in H.
-    destruct bv as [bv bv_wf].
-    simpl in *.
-    funelim (XBV.to_bv xbv).
-    + unfold XBV.raw_to_bv_with_proof in *.
-      rewrite e in Heq. inv Heq.
-      f_equal.
-      apply BV.of_bits_equal.
-      simpl. destruct_rew.
-      destruct v as [v v_wf].
-      unfold XBV.bits, XBV.bv, RawBV.of_bits in *. simpl in *. subst.
-      rewrite RawXBV.xbv_bv_inverse in e.
-      inv e.
-      reflexivity.
-    + destruct v as [v v_wf].
-      simpl in *. subst.
-      clear Heq.
-      rewrite RawXBV.xbv_bv_inverse in prf.
-      discriminate.
-Qed.
 
 Lemma select_bit_to_bv w_vec w_idx (vec : BV.bitvector w_vec) (idx : BV.bitvector w_idx) :
   (BV.to_N idx < w_vec)%N ->
@@ -996,9 +117,9 @@ Proof.
   intros H.
   unfold select_bit, select_bit_bv.
   rewrite XBV.to_N_from_bv.
-  rewrite bit_of_as_bv by lia.
+  rewrite XBV.bit_of_as_bv by lia.
   generalize (BV.bitOf (n:=w_vec) (N.to_nat (BV.to_N idx)) vec). intro b.
-  apply to_bv_some_raw_iff.
+  apply XBV.to_bv_some_raw_iff.
   simpl.
   unfold RawXBV.to_bv. simpl.
   rewrite RawXBV.bit_to_bool_inverse.
@@ -1034,57 +155,6 @@ Proof.
     eauto using XBV.to_N_max_bound.
 Qed.
 
-Lemma rawxbv_from_bv_app b1 b2 :
-  RawXBV.from_bv (b1 ++ b2)%list = (RawXBV.from_bv b1 ++ RawXBV.from_bv b2)%list.
-Proof. unfold RawXBV.from_bv. apply List.map_app. Qed.
-
-
-(* Move me to common *)
-Lemma map_removelast {A B} (f : A -> B) (l : list A) :
-  List.map f (List.removelast l) = List.removelast (List.map f l).
-Proof.
-  induction l; simpl; [reflexivity|].
-  destruct l; simpl in *; [reflexivity|].
-  now rewrite IHl.
-Qed.
-
-Lemma shl_to_bv n vec shamt :
-  XBV.to_bv (XBV.shl (XBV.from_bv vec) shamt) = Some (BV.shl (n:=n) vec shamt).
-Proof.
-  unfold BV.to_N, BV.shl.
-  intros.
-  destruct vec as [vec vec_wf].
-  rewrite <- XBV.xbv_bv_inverse. f_equal.
-  apply XBV.of_bits_equal; simpl.
-  generalize dependent (N.to_nat shamt). clear shamt. intro shamt.
-  funelim (RawBV.shl vec shamt).
-  - reflexivity.
-  - reflexivity.
-  - insterU H.
-    unfold RawXBV.from_bv in *. cbn [List.map].
-    simp shl. repeat f_equal.
-    rewrite map_removelast in *.
-    cbn [List.map] in H.
-    apply H.
-Qed.
-
-Lemma shr_to_bv n vec shamt :
-  XBV.to_bv (XBV.shr (XBV.from_bv vec) shamt) = Some (BV.shr (n:=n) vec shamt).
-Proof.
-  unfold BV.to_N, BV.shr.
-  intros.
-  destruct vec as [vec vec_wf].
-  rewrite <- XBV.xbv_bv_inverse. f_equal.
-  apply XBV.of_bits_equal; simpl.
-  generalize dependent (N.to_nat shamt). clear shamt. intro shamt.
-  funelim (RawBV.shr vec shamt); simpl; simp shr.
-  - reflexivity.
-  - reflexivity.
-  - unfold RawXBV.from_bv in *.
-    rewrite List.map_app. simpl. repeat f_equal.
-    eauto.
-Qed.
-
 Lemma var_to_smt_value var (m : VerilogSMTBijection.t) tag regs ρ t :
     var_to_smt tag m var = inr t ->
     verilog_smt_match_states_partial (fun v => v = var) tag m regs ρ ->
@@ -1113,22 +183,6 @@ Proof.
   intros Htransf Hsat.
   funelim (var_to_smt tag m var); rewrite <- Heqcall in *; monad_inv.
   crush.
-Qed.
-
-Lemma bitOf_in_bounds n w (bv : BV.bitvector w) def :
-  (n < w)%N ->
-  RawXBV.bit_to_bool (XBV.bitOf (N.to_nat n) (XBV.from_bv bv)) = Some (List.nth (N.to_nat n) (BV.bits bv) def).
-Proof.
-  intros H.
-  destruct bv as [bv wf].
-  unfold XBV.from_bv, RawXBV.from_bv, XBV.bitOf, RawXBV.bitOf,
-    BVList.RAWBITVECTOR_LIST.size in *.
-  subst. simpl.
-  erewrite List.nth_indep
-    by (rewrite List.length_map; lia).
-  rewrite List.map_nth.
-  rewrite RawXBV.bit_to_bool_inverse.
-  reflexivity.
 Qed.
 
 Lemma select_bit_no_exes:
@@ -1160,7 +214,7 @@ Proof.
   funelim (convert w_to (XBV.from_bv from));
     try destruct_rew; clear Heqcall.
   - rewrite XBV.zeros_from_bv.
-    rewrite xbv_concat_no_exes. simpl.
+    rewrite XBV.concat_no_exes. simpl.
     funelim (convert_bv (to - from + from) from0); [|lia|lia].
     clear Heqcall.
     apply XBV.of_bits_equal.
@@ -1223,17 +277,17 @@ Proof.
   - (* shift right *)
     rewrite XBV.to_N_from_bv.
     simpl.
-    rewrite shr_to_bv.
+    rewrite XBV.shr_to_bv.
     eauto.
   - (* shift left *)
     rewrite XBV.to_N_from_bv.
     simpl.
-    rewrite shl_to_bv.
+    rewrite XBV.shl_to_bv.
     eauto.
   - (* shift left (arithmetic) *)
     rewrite XBV.to_N_from_bv.
     simpl.
-    rewrite shl_to_bv.
+    rewrite XBV.shl_to_bv.
     eauto.
 Qed.
 
@@ -1348,7 +402,7 @@ Proof.
     rewrite select_bit_no_exes by assumption.
     eauto.
   - (* concat *)
-    rewrite xbv_concat_no_exes.
+    rewrite XBV.concat_no_exes.
     eauto.
   - (* literal *)
     eauto.
@@ -1430,16 +484,16 @@ Proof.
     simpl; rewrite Hinterp_lhs; rewrite Hinterp_rhs; autodestruct; try contradiction;
     repeat f_equal; rewrite <- eq_rect_eq.
   - rewrite XBV.to_N_from_bv in *. simpl in *.
-    erewrite shr_to_bv in *.
-    rewrite bv_shr_swap_definition.
+    erewrite XBV.shr_to_bv in *.
+    rewrite BV.shr_swap_definition.
     now some_inv.
   - rewrite XBV.to_N_from_bv in *. simpl in *.
-    erewrite shl_to_bv in *.
-    rewrite bv_shl_swap_definition.
+    erewrite XBV.shl_to_bv in *.
+    rewrite BV.shl_swap_definition.
     now some_inv.
   - rewrite XBV.to_N_from_bv in *. simpl in *.
-    erewrite shl_to_bv in *.
-    rewrite bv_shl_swap_definition.
+    erewrite XBV.shl_to_bv in *.
+    rewrite BV.shl_swap_definition.
     now some_inv.
 Qed.
 
@@ -1518,31 +572,6 @@ Proof.
     apply value_bitvec_bits_equal.
     destruct_rew.
     reflexivity.
-Qed.
-
-Lemma bv_shr_as_select w (vec : BV.bitvector w) (idx : BV.bitvector w) :
-  (w > 0)%N ->
-  BV.bv_extr 0 1 (BV.bv_shr vec idx) =
-    BV.of_bits [BV.bitOf (N.to_nat (BV.to_N idx)) vec]%list.
-Proof.
-  intros Hbound.
-  rewrite bv_extr_one_bit; try crush.
-  apply BV.of_bits_equal. simpl.
-  do 2 f_equal.
-  unfold BV.bitOf, BV.bv_shr.
-  destruct vec as [vec vec_wf].
-  destruct idx as [idx idx_wf].
-  simpl.
-  unfold BV.to_N, RawBV.to_N, BV.bv_shr, RawBV.bv_shr, RawBV.shr_be, RawBV.size in *.
-  simpl.
-  rewrite vec_wf, idx_wf, N.eqb_refl.
-  generalize (RawBV.list2nat_be idx). clear idx idx_wf. intro n.
-  destruct n, vec; try crush.
-  unfold RawBV.bitOf.
-  rewrite RawBV.shr_be_nicify. simp nice_nshr_be. rewrite Nat2N.id. simpl.
-  clear b vec_wf.
-  funelim (RawBV.nice_nshr_be vec n); simp nice_nshr_be; try crush.
-  destruct (RawBV.nice_nshr_be bs n); crush.
 Qed.
 
 Lemma to_N_convert_bv_extn from to (bv : BV.bitvector from) :
@@ -1629,14 +658,14 @@ Proof.
   erewrite ! cast_from_to_value; cycle 1;
     try eassumption; try lia; [idtac].
   destruct (N.eq_dec (N.max w_vec w_idx) (N.max w_vec w_idx)); [|crush].
-  rewrite bv_shr_as_select by lia.
-  rewrite bit_of_as_bv in Heval by lia.
+  rewrite BV.bv_shr_as_select by lia.
+  rewrite XBV.bit_of_as_bv in Heval by lia.
   do 2 f_equal.
   destruct_rew.
   rewrite to_N_convert_bv_extn by lia.
   rewrite bitOf_convert_bv_extn by lia.
   (* Ugly, but it's hard to extract a lemma - the widths don't match up *)
-  apply to_bv_some_raw_iff in Heval. simpl in Heval.
+  apply XBV.to_bv_some_raw_iff in Heval. simpl in Heval.
   apply BV.of_bits_equal. simpl.
   unfold RawXBV.to_bv, RawBV.of_bits in *; simpl in *.
   rewrite RawXBV.bit_to_bool_inverse in Heval.
@@ -1650,7 +679,7 @@ Lemma convert_extend_to_N from to (xbv : XBV.xbv from) val :
 Proof.
   intros.
   funelim (convert to xbv); [idtac|lia|idtac].
-  - destruct_rew. simpl. apply extend_to_N. assumption.
+  - destruct_rew. simpl. apply XBV.extend_to_N. assumption.
   - destruct_rew. simpl. assumption.
 Qed.
 
@@ -1661,7 +690,7 @@ Lemma convert_extend_to_N_none from to (xbv : XBV.xbv from) :
 Proof.
   intros.
   funelim (convert to xbv).
-  - destruct_rew. simpl. apply extend_to_N_none2. assumption.
+  - destruct_rew. simpl. apply XBV.extend_to_N_none2. assumption.
   - lia.
   - destruct_rew. simpl. assumption.
 Qed.
@@ -1674,7 +703,7 @@ Proof.
   funelim (convert n2 xbv); [idtac|lia|idtac].
   - destruct_rew. simpl.
     funelim (convert from (XBV.shr (XBV.concat (XBV.zeros (to - from)) value) shamt)); [lia|idtac|lia].
-    apply extr_shr_extend.
+    apply XBV.extr_shr_extend.
   - destruct_rew. simpl.
     funelim (convert from (XBV.shr value shamt)); [lia|lia|idtac].
     rewrite <- eq_rect_eq. reflexivity.
@@ -1688,7 +717,7 @@ Proof.
   funelim (convert n2 xbv); [idtac|lia|idtac].
   - destruct_rew. simpl.
     funelim (convert from (XBV.shl (XBV.concat (XBV.zeros (to - from)) value) shamt)); [lia|idtac|lia].
-    apply extr_shl_extend.
+    apply XBV.extr_shl_extend.
   - destruct_rew. simpl.
     funelim (convert from (XBV.shl value shamt)); [lia|lia|idtac].
     rewrite <- eq_rect_eq. reflexivity.
@@ -1701,7 +730,7 @@ Proof.
   intros. 
   funelim (convert n2 (XBV.exes n1)).
   - lia.
-  - apply extr_exes.
+  - apply XBV.extr_exes.
   - destruct_rew. reflexivity.
 Qed.
 
@@ -1898,7 +927,7 @@ Proof.
     replace (eval_expr regs expr2) in *.
     simpl in *.
     rewrite XBV.xbv_bv_inverse in *.
-    rewrite xbv_concat_to_bv.
+    rewrite XBV.concat_to_bv.
     inv Hexpr_to_smt.
     simpl.
     rewrite IHexpr1, IHexpr2.
